---
title:
date: 2021-09-11 16:26
tags: []

---

### 09/11/2021

![image-20210911173532220](/assets/images/2021-09/image-20210911163103702.png)

#### Calculate the total length of segments in red color.

**Solve 1:**

Using [Descartes's Theorem](https://en.wikipedia.org/wiki/Descartes%27_theorem),

Four circles centered at $O, r_0, r_1, r_2$ are tangent to each other, so

$2(\dfrac{1}{2^2}+\dfrac{1}{1}+\dfrac{1}{1}+\dfrac{1}{r_2^2})=(-\dfrac{1}{2}+\dfrac{1}{1}+\dfrac{1}{1}+\dfrac{1}{r_2})^2 \implies r_2=\dfrac{2}{3}$

Four circles centered at $O, r_0, r_2, r_3$ are tangent to each other, so

$2(\dfrac{1}{2^2}+\dfrac{1}{1}+\dfrac{3^2}{2^2}+\dfrac{1}{r_3^2})=(-\dfrac{1}{2}+\dfrac{1}{1}+\dfrac{3}{2}+\dfrac{1}{r_3^2})^2 \implies r_3=\dfrac{1}{3}$

And Four circles centered at $O, r_0, r_{n-1},r_{n}$ are tangent to each other, so

$2(\dfrac{1}{2^2}+\dfrac{1}{1}+\dfrac{1}{r_{n-1}^2}+\dfrac{1}{r_n^2})=(-\dfrac{1}{2}+\dfrac{1}{1}+\dfrac{1}{r_{n-1}}+\dfrac{1}{r_n})^2$

Four circles centered at $O, r_0, r_{n-2}, r_{n-1}$ are tangent to each other, so

$2(\dfrac{1}{2^2}+\dfrac{1}{1}+\dfrac{1}{r_{n-2}^2}+\dfrac{1}{r_{n-1}^2})=(-\dfrac{1}{2}+\dfrac{1}{1}+\dfrac{1}{r_{n-2}}+\dfrac{1}{r_{n-1}})^2$

In above two equations, take $c_{n-1}=\dfrac{1}{r_{n-1}}$ as known value,

and take $c_{n-2}=\dfrac{1}{r_{n-2}}, c_n=\dfrac{1}{r_n}$ as two solutions of variable $x$, then we get the equation

$2(\dfrac{1}{2^2}+\dfrac{1}{1}+c_{n-1}^2+x^2)=(-\dfrac{1}{2}+\dfrac{1}{1}+c_{n-1}+{x})^2$

$\implies x^2-(2c_{n-1}+1)x+(c_{n-1}^2-c_{n-1}+\dfrac{9}{4})=0$

Via [Vieta's Formula](https://en.wikipedia.org/wiki/Vieta%27s_formulas) we know that

$c_{n-2}+c_n=2c_{n-1}+1 \implies c_n-c_{n-1}=c_{n-1}-c_{n-2}+1$

Let $d_n\triangleq c_n-c_{n-1} \implies d_n=d_{n-1}+1$

$r_1=1, r_2=\dfrac{2}{3} \implies c_1=1, c_2=\dfrac{3}{2} \implies d_2=\dfrac{1}{2} \implies d_n=d_2+(n-2)=\dfrac{1}{2}+(n-2) \implies c_n-c_{n-1}=n-\dfrac{3}{2}$

$\implies c_n=d_n+c_{n-1}=d_n+d_{n-1}+c_{n-2}=...=\displaystyle \sum_{i=2}^{n}{d_i}+c_1=\displaystyle \sum_{i=2}^{n}{(i-\dfrac{3}{2})}+1$

$=\displaystyle \sum_{i=2}^{n}{i}-(n-1)\dfrac{3}{2}+1=\dfrac{n(n+1)}{2}-1-\dfrac{3n-3}{2}+1=\dfrac{n^2-2n+3}{2}$

$\implies r_n=\dfrac{1}{c_n}=\dfrac{2}{n^2-2n+3}$

The total length of segments is

$\displaystyle 2\sum_{i=1}^{\infty}{r_i}-r_1= 2\sum_{i=1}^{\infty}{\dfrac{2}{i^2-2i+3}}-1=4\sum_{i=1}^{\infty}{\dfrac{1}{(i-1)^2+2}}-1=4\sum_{i=0}^{\infty}{\dfrac{1}{i^2+2}}-1$

Now the task is to calculate the sum of infinite series.

$\dfrac{sin(\pi x)}{\pi x}=\displaystyle \prod_{n=1}^{\infty}{(1-\dfrac{x^2}{n^2})} \implies [ln\dfrac{sin(\pi x)}{\pi x}]'=\sum_{n=1}^{\infty}{ln[(1-\dfrac{x^2}{n^2})]'}$

$\implies \dfrac{\pi x}{sin(\pi x)}\cdot\dfrac{\pi cos(\pi x)\cdot \pi x -\pi sin(\pi x)} {(\pi x)^2}=\dfrac{\pi cos(\pi x)}{sin(\pi x)}-\dfrac{1}{x}=\displaystyle \sum_{n=1}^{\infty}{\dfrac{n^2}{n^2-x^2}\cdot(\dfrac{-2x}{n^2})}=-\sum_{n=1}^{\infty}{\dfrac{2x}{n^2-x^2}}$

$\implies \displaystyle \sum_{n=1}^{\infty}{\dfrac{1}{n^2-x^2}}=\dfrac{1}{2x^2}-\dfrac{\pi cot(\pi x)}{2x}$

Let $x=-ik \implies \displaystyle \sum_{n=1}^{\infty}{\dfrac{1}{n^2+k^2}}=-\dfrac{1}{2k^2}+\dfrac{\pi cot(-i k \pi)}{2ik}$

Use equity $cot (x) = i cot (ix) \implies \displaystyle \sum_{n=1}^{\infty}{\dfrac{1}{n^2+k^2}}=-\dfrac{1}{2k^2}+\dfrac{\pi cot(k\pi )}{2k}$

So the total length of segments is:

$4\displaystyle \sum_{i=0}^{\infty}{\dfrac{1}{i^2+(\sqrt{2})^2}}-1=4(\dfrac{1}{2}-\dfrac{1}{2*(\sqrt{2})^2}+\dfrac{\pi cot(\sqrt{2}\pi)}{2\sqrt{2}})-1=\sqrt{2}\pi cot(\sqrt{2} \pi)$

$=\sqrt{2}\pi\dfrac{exp(\sqrt{2}\pi)+exp(-\sqrt{2}\pi)}{exp(\sqrt{2}\pi)-exp(-\sqrt{2}\pi)}\approx 4.4441$

**Solve 2:**



**Note for reading:**

* https://zh.wikipedia.org/wiki/%E7%AE%97%E9%A1%8D
* https://zh.wikipedia.org/wiki/%E7%B9%AA%E9%A6%AC
* https://en.wikipedia.org/wiki/Pappus_chain
* https://en.wikipedia.org/wiki/Arbelos
* https://en.wikipedia.org/wiki/Inversive_geometry
* https://www.math.tamu.edu/~harold.boas/preprints/arbelos.pdf
* http://jwilson.coe.uga.edu/MATH7200/InversionCompanion/inversion/inversionSupplement.pdf

