---
title: July 2021 Monthly Problems
date: 2021-07-04 11:35
tags: []
---

### 07/03/2021

![image-20210704115651739](/assets/images/2021-07/image-20210704115651739.png)

#### Solve angle $x$.

**Solve 1：**

![image-20210630103353402](/assets/images/2021-07/image-20210630103353402.png)

Make $ABCE$ a square. Connect $BE$. $BE$ and $AC$ intersect at $F$. Connect $DE$. $DE$ and $AC$ intersect at $H$.

Easy to see by symmetry that $\angle{ADB}=\angle{EDC}, \angle{DAC}=\angle{DEB}$, and $\triangle{BCF}$ is also an isosceles right triangle, $BF=EF=FC$

Make $G$ inside it so that $\angle{GBF}=\angle{GFB}=\angle{BCG}$, then we know $\angle{GCB}=\angle{DCB} \implies$ $C,D,G$ is collinear.

Connect $GH$, since $\angle{DAC}=\angle{DEB}=\angle{GBF}$, we know that $B,G,H$ is collinear.

Connect $DF$. Easy to see from symmetry that $\angle{DFC}=45^{\circ}$, $\angle{HGC}=\angle{GBC}+\angle{GCB}=\angle{GBC}+\angle{GBF}=45^{\circ}$

$\implies G,D,H,F$ are cyclic $\implies \angle{GFD}=\angle{GHD}$

$\angle{BFG}=\angle{BED} \implies FG \parallel DE \implies \angle{FGH}=\angle{GHD} \implies \angle{GFD}=\angle{FGH}=\angle{GBF}+\angle{BFG}$

$\implies \angle{BFD}=45^{\circ}=\angle{BFG}+\angle{GBF}+\angle{BFG}=3\cdot\angle{BFG} \implies \angle{BFG}=15^{\circ}$

$\implies \angle{CAD}=\angle{BFG}=\angle{BCD}=\boxed{15^{\circ}}$

**Solve 2:**

![image-20210630185311870](/assets/images/2021-07/image-20210630185311870.png)

$\angle{DAC}=x, \angle{ACD}=45^{\circ}-x \implies \angle{ADC}=135^{\circ}$

Let $E$ be the circumcenter of $\triangle{ACD}$, easy to know that

$EA=ED=EC, \angle{AEC}=(180^{\circ}-135^{\circ}) * 2=90^{\circ}$

So $ABCE$ is a square

$AB=CE, BD=CD, \angle{ABD}=\angle{ECD} \implies \triangle{ABD} \cong \triangle{ECD}$

$\implies EA=ED=EC=AB=CD \implies \angle{AED}=60^{\circ}$

$\implies \angle{DEC}=90^{\circ}-60^{\circ}=30^{\circ}\implies \angle{DAC}=\dfrac{1}{2}\angle{DEC}=\boxed{15^{\circ}}$

**Solve 3:**

![image-20210701020610025](/assets/images/2021-07/image-20210701020610025.png)

$\angle{DAC}=x, \angle{ACD}=45^{\circ}-x \implies \angle{ADC}=135^{\circ}$

Let $AB=AC=a, BD=CD=b$

In $\triangle{ACD}$: $\dfrac{AC}{sin135^{\circ}}=\dfrac{CD}{sinx} \implies 2a*sinx=b$

In $\triangle{BCD}$: $\dfrac{BC}{sin(2x)}=\dfrac{BD}{sinx}\implies a*sinx=b*sin(2x)=2a*sinx*sin(2x)$

$\implies sin(2x)=\dfrac{1}{2}\implies 2x=30^{\circ} \implies x=\boxed{15^{\circ}}$

**Solve4:**

From [Trigonometric Form of Ceva's Theorem](https://www.cut-the-knot.org/triangle/TrigCeva.shtml)

$\dfrac{sin(45^{\circ}-x)}{sinx}\dfrac{sin(45^{\circ}-x)}{sinx}\dfrac{sinx}{sin(90^{\circ}-x)}=1$

$\implies sin^2(45^{\circ}-x)=sinx*cosx$

$\implies (sin45^{\circ}cosx-cos45^{\circ}sinx)^2=sinx*cosx$

$\implies 4sinx*cosx=1 \implies sin(2x)=\dfrac{1}{2} \implies 2x=30^{\circ}\implies x=\boxed{15^{\circ}}$

---

### 07/04/2021

![image-20210703140239428](/assets/images/2021-07/image-20210703140239428.png)

#### Solve angle $x$.

**Solve:**

![image-20210703140056114](/assets/images/2021-07/image-20210703140056114.png)

Draw $MD \perp AD$ and $MD=CD=1$, easy to see that $AM=2, \angle{CDM}=30^{\circ} \implies \angle{MCD}=75^{\circ}$

Draw $AO\perp MO$ and $AO=MO$, easy to see that $AO=MO=\sqrt{2}$

$cos(\angle{ADC})=cos120^{\circ}=\dfrac{AD^2+CD^2-AC^2}{2*CD*AD}=\dfrac{4-AC^2}{2\sqrt{3}}=-\dfrac{1}{2} \implies AC^2=4+\sqrt{3}$

$\implies CO^2=AC^2-AO^2=4+\sqrt{3}-2=2+\sqrt{3}$

$cos(\angle{CDM})=cos30^{\circ}=\dfrac{CD^2+MD^2-CM^2}{2*CD*MD}=\dfrac{2-CM^2}{2}=\dfrac{\sqrt{3}}{2}\implies CM^2=2-\sqrt{3}$

$\implies CM^2=\dfrac{4-2\sqrt{3}}{2}=\dfrac{(\sqrt{3}-1)^2}{2}\implies CM=\dfrac{\sqrt{3}-1}{\sqrt{2}}$

$\implies (CM+MO)^2=(\dfrac{\sqrt{3}-1}{\sqrt{2}}+\sqrt{2})^2=(\dfrac{\sqrt{3}-1+2}{\sqrt{2}})^2=\dfrac{4+2\sqrt{3}}{2}=2+\sqrt{3}=CO^2$

$\implies CM+MO=CO \implies C,M,O$ are collinear $\implies \triangle{ABC}\cong \triangle{AOC}$

$\implies OC\perp BC \implies \angle{BCD}=90^{\circ}-\angle{DCM}=\boxed{15^{\circ}}$

---

### 07/14/2021

#### $\triangle{ABC}$ is equilateral triangle. Point $D$ is outside the triangle and $AD=AB, \angle{DAB}=36^{\circ}$. Point $E$ is on $BD$ and $AE\perp BD$. $F$ is a point on $AE$ so that $\angle{BFC}=72^{\circ}$ and $AF$ is as short as possible. Prove $DF=FB=DB$

![image-20210714143737213](/assets/images/2021-07/image-20210714143737213.png)

**Prove:**

---

### 07/25/2021

#### $\triangle{ABC}$ is equilateral. Points $E,F,G$ are inside it and form four triangles so that $S_c=S_a=S_b=S_4$. Find $\dfrac{AF}{FG}$.

![image-20210725002311360](/assets/images/2021-07/image-20210725002311360.png)

**Solve:**

Choose Barycentric coordinate, $A(1,0,0), B(0,1,0), C(0,0,1)$

Let $S_{\triangle{BCG}}=S_a, S_{\triangle{ACE}}=S_b, S_{\triangle{ABF}}=S_c, S_{\triangle{ABC}}=S$, then

$E(\dfrac{1}{4}, \dfrac{S_b}{S}, \dfrac{3}{4}-\dfrac{S_b}{S}), F(\dfrac{3}{4}-\dfrac{S_c}{S}, \dfrac{1}{4}, \dfrac{S_c}{S}), G(\dfrac{S_a}{S}, \dfrac{3}{4}-\dfrac{S_a}{S}, \dfrac{1}{4})$​
$$
\begin{align*}
 CEF \text{ collinear } \implies \begin{vmatrix} \dfrac{3}{4}-\dfrac{S_c}{S} & \dfrac{1}{4} & 1 \\ \dfrac{1}{4} & \dfrac{S_b}{S} & 1 \\ 0 & 0 & 1 \end{vmatrix}=0 \implies 16S_bS_c-12SS_b+S^2=0 \implies S_c=\dfrac{3}{4}S-\dfrac{S^2}{16S_b}\\
 BGE \text { collinear } \implies \begin{vmatrix} \dfrac{1}{4} & \dfrac{S_b}{S} & 1 \\ \dfrac{S_a}{S} & \dfrac{3}{4}-\dfrac{S_a}{S} & 1 \\ 0 & 0 & 1 \end{vmatrix}=0 \implies 16S_aS_b-12SS_a+S^2=0 \implies S_a=\dfrac{3}{4}S-\dfrac{S^2}{16S_c}\\
 AFG \text{ collinear } \implies \begin{vmatrix} \dfrac{3}{4}-\dfrac{S_c}{S} & \dfrac{1}{4} & 1 \\ \dfrac{S_a}{S} & \dfrac{3}{4}-\dfrac{S_a}{S} & 1 \\ 1 & 0 & 1 \end{vmatrix}=0 \implies 16S_cS_a-12SS_c+S^2=0 \implies S_b=\dfrac{3}{4}S-\dfrac{S^2}{16S_a}\\
\end{align*}
$$
$\implies S_c=\dfrac{3}{4}S-\dfrac{S^2}{16(\dfrac{3}{4}S-\dfrac{S^2}{16S_a})}=\dfrac{3}{4}S-\dfrac{S}{12-\dfrac{S}{S_a}}=\dfrac{3}{4}S-\dfrac{S}{12-\dfrac{S}{\dfrac{3}{4}S-\dfrac{S^2}{16S_c}}}=\dfrac{3}{4}S-\dfrac{(12S_c-S)S}{128S_c-12S}$

$\implies 16S_c^2-12S_cS+S^2=0\implies S_c=\dfrac{3-\sqrt{5}}{8}S$ (remove the situation $S_c=\dfrac{3+\sqrt{5}}{8}S$)​

$\implies S_a=\dfrac{3}{4}S-\dfrac{S^2}{16S_c}=\dfrac{3}{4}S-\dfrac{S^2}{16\dfrac{3-\sqrt{5}}{8}S}=\dfrac{3-\sqrt{5}}{8}S \implies S_b=\dfrac{3-\sqrt{5}}{8}S$​

$\implies S_a=S_b=S_c$​ (this step is to prove the symmetric conclusion that people take for granted)

$S_1=\dfrac{1}{4}S=S_c+S_{\triangle{BFG}}=\dfrac{3-\sqrt{5}}{8}S+S_{\triangle{BFG}}\implies S_{\triangle{BFG}}=\dfrac{\sqrt{5}-1}{8}S$

$\implies \dfrac{AF}{FG}=\dfrac{S_c}{S_{\triangle{BFG}}}=\dfrac{3-\sqrt{5}}{\sqrt{5}-1}=\boxed{\dfrac{\sqrt{5}-1}{2}}$​​

