---
title:
date: 2021-12-03 04:35
tags: []
---
### 12/03/2021

#### Two green circles are externally tangent and two purple circles are externally tangent at the same point. And all these four circles are internally tangent to a blue circle. The radiuses of the green circles are 3 and 4. The radius of one purple circle is 2. Find the radius of the other purple circle.

**Solve:**

![image-20211203043954896](/assets/images\2021-12/image-20211203043700833.png)

Let $A, B$ be the centers of two green circles, $C,D$ the centers of two purple circles, $O$ the tangent point. Let circle $O$ be the unit circle centered at $O$. Get the inversions of all the circles:

![image-20211203045834580](/assets/images/2021-12/image-20211203045834580.png)

Due to the properties of inversion, the green circles pass through the inversion center $O$, so they are converted to line $a, b$, with distances to $O$ as $\dfrac{1}{2r_A}, \dfrac{1}{2r_B}$ respectively; similarly, the purple circles are converted to line $c,d$ with distances to $O$ as $\dfrac{1}{2r_C}, \dfrac{1}{2r_D}$ respectively. The blue circle does not pass through the inversion center $O$ so it is converted to a circle, still tangent to the mirrors of the four circles, i.e., four lines $a,b,c,d$. So we know that the distance between line $a,b$ is equal to the distance between line $c,d$:

$\dfrac{1}{2r_A}+\dfrac{1}{2r_B}=\dfrac{1}{2r_C}+\dfrac{1}{2r_D} \implies \dfrac{1}{r_A}+\dfrac{1}{r_B}=\dfrac{1}{r_C}+\dfrac{1}{r_D}$

$r_A=3, r_B=4, r_C=2 \implies r_D=\boxed{12}$

So the radius of the other purple circle is 12.

#### [中文] 两个相互外切的绿色圆与两个相互外切的紫色圆的切点在同一点，这四个圆与蓝色圆内切。已知绿色圆半径为3和4，其一紫色圆半径为2，求另一紫色圆半径。

![image-20211203043954896](/assets/images\2021-12/image-20211203043700833.png)

**解：**

设绿色圆圆心$A,B$和紫色圆圆心$C,D$以及切点$O$如上图所示。做以$O$为圆心的单位圆（下图红色圆），对所有五个圆做关于该单位圆的反演变换：

![image-20211203045834580](/assets/images/2021-12/image-20211203045834580.png)

根据反演变换性质易知，绿圆$A,B$经过反演中心$O$，所以它们关于单位圆$O$的像为直线$a,b$，与反演中心$O$的距离分别为$\dfrac{1}{2r_A}, \dfrac{1}{2r_B}$，紫圆$C,D$也经过反演中心$O$，所以它们关于单位圆$O$的像为直线$c,d$，与反演中心的距离分别为$\dfrac{1}{2r_C}, \dfrac{1}{2r_D}$。蓝圆与四圆相切，且不经过反演中心$O$，所以它关于单位圆$O$的像仍然为圆，且与四圆的像相切，即为上图所示虚线蓝圆，可见直线$a,b$的相距与直线$c,d$的相距相等，即

$\dfrac{1}{2r_A}+\dfrac{1}{2r_B}=\dfrac{1}{2r_C}+\dfrac{1}{2r_D} \implies \dfrac{1}{r_A}+\dfrac{1}{r_B}=\dfrac{1}{r_C}+\dfrac{1}{r_D}$

$r_A=3, r_B=4, r_C=2 \implies r_D=\boxed{12}$

故所求紫色圆半径为12。

---

### 12/04/2021

#### Rectangle $ABCD$ has two points $E, F$ on side $BC, CD$, and $\triangle{AEF}$ is equilateral. Prove $S_{\triangle{CEF}}=S_{\triangle{ADF}}+S_{\triangle{ABE}}$

![image-20211204154952844](/assets/images/2021-12/image-20211204154952844.png)

**Prove:**

![image-20211204155536966](/assets/images/2021-12/image-20211204155536966.png)

Let $S_{\triangle{AEF}}=S_0, S_{\triangle{ADF}}=S_1, S_{\triangle{ABE}}=S_2, S_{\triangle{CEF}}=S_3$. So we need prove $S_3=S_1+S_2$.

Extend $AB$ to $A'$ so that $AB=BA'$, extend $DC$ to $D'$ so that $DC=CD'$. Extended $AE$ and $A'D'$ intersect at $G$. Connect $FG$.

Easy to see that $AB=BA' \implies AE=EG \implies S_{\triangle{AEF}}=S_{\triangle{FEG}}=S_0, S_{EBA'G}=3S_{\triangle{ABE}}=3S_2$

 $\angle{FAE}=60^{\circ}, AE=EF=AF \implies \angle{EFG}=\angle{AGF}=30^{\circ} \implies \angle{AFG}=90^{\circ}, GF=\sqrt{3}AF $

$\implies \angle{DAF}=\angle{D'FG} \implies S_{\triangle{D'FG}}=3S_{\triangle{ADF}}=3S_1$

$\implies S_{AA'D'D}=2S_{ABCD}=2(S_0+S_1+S_2+S_3)=2S_0+S_1+3S_1+4S_2 \implies S_3=S_1+S_2 \blacksquare$

---

### 12/05/2021

#### Given any five integers, prove that there must be four of them as $a,b,c,d$ so that 28 divides $(a^2-b^2)(c^2-d^2)$

**Proof:**
All integers mod by $7$ we get  ${0, 1, 2, 3, 4, 5, 6}$, so their squares mod by $7$ will be ${0, 1, 4, 9\equiv 2, 16 \equiv 2, 25 \equiv 4, 36 \equiv 1}={0, 1, 2, 4}$.

So pick any $5$ from them will at least have two integers that the difference of their squares is $0$ mod 7. Take them as $a, b$.

All integers mod by $4$ we get $0, 1, 2, 3$, so their squares mod by $4$ will be ${0, 1, 4 \equiv 0, 9 \equiv 1}={0, 1}$. For the rest of the three integers after above step, there must be two of them so that the difference of their squares is $0$ mod 4. Take them as $c, d$.

So there will be $(a^2-b^2)(c^2-d^2) \equiv 0$ mod $28$. $\blacksquare$

---

### 12/06/2021

#### In $\triangle{ACD}, \angle{A}=84^{\circ}, \angle{ACD}=42^{\circ}$. Now extend $AD$ to $B$ so that $AC=BD$. Find $\angle{BCD}$.

![The Figure of Problem](/assets/images/2021-12/image-20211206161293.png)

**Solve 1:**

![image-20211206164152087](/assets/images/2021-12/image-20211206161534149.png)

Make $A'$ on $AD$ so that $\angle{ACA'}=12^{\circ} \implies AC=A'C, \angle{A'AC}=84^{\circ}, \angle{ACD}=30^{\circ}$.

Let $E$ be the circumcenter of $\triangle{A'CD} \implies A'E=CE=DE, \angle{CED}=2*\angle{A'AC}=168^{\circ} \implies \angle{EDC}=\angle{ECD}=6^{\circ}$

$\implies \angle{EDA'}=54^{\circ}+6^{\circ}=60^{\circ} \implies \triangle{A'DE}$ is equilateral triangle.

Make equilateral $\triangle{A'CF}$, so that $A'C=CF=A'F=BD$, $A'F$ and $CG$ intersect at $G$. Easy to see that $CG \perp A'F \implies DF=A'D, \angle{DFA'}=\angle{DA'F}=\angle{EA'C}=\angle{ECA'}=36^{\circ}$

Now make $H$ on $A'C$ so that $CE=CH=DE=A'E \implies \angle{CHE}=\angle{CEH}=72^{\circ} \implies \angle{EA'H}=\angle{A'EH}=36^{\circ} \implies A'H=EH$

$\implies \triangle{A'DF} \sim \triangle{A'EC} \implies \dfrac{A'D}{AF}=\dfrac{A'H}{A'E} \implies \dfrac{A'D+AF}{AF}=\dfrac{A'H+A'E}{A'E} \implies \dfrac{A'D+BD}{AC}=\dfrac{A'H+CH}{A'D}$

$\implies \dfrac{A'B}{A'C}=\dfrac{A'C}{A'D}\implies \triangle{A'BC} \sim \triangle{A'CD} \implies \angle{A'BC}=\angle{A'CD}=30^{\circ} \implies \angle{BCD}=54^{\circ}-30^{\circ}=\bbox[5px, border: 1px solid black]{24^{\circ}} $

**Solve 2:**

![image-20211206181238385](/assets/images/2021-12/image-20211206181238385.png)

Make $A'$ on $AD$ so that $\angle{ACA'}=12^{\circ} \implies AC=A'C, \angle{A'AC}=84^{\circ}, \angle{ACD}=30^{\circ}$.

Make equilateral $\triangle{A'CF}$, so that $A'C=CF=A'F=BD$, $A'F$ and $CG$ intersect at $G$. Easy to see that $CG \perp A'F \implies DF=A'D, \angle{DFA'}=\angle{DA'F}=36^{\circ} \implies \angle{BDF}=72^{\circ}$

Make $D'$ on $BD$ so that $FD'=FD \implies \angle{DD'F}=72^{\circ} \implies \angle{DFD'}=36^{\circ}\implies\angle{AD'F}=\angle{A'FD'}=72^{\circ} $

$\implies A'F=A'D'=AC=BD \implies BD'=A'D=FD=FD'\implies \angle{D'BF}=36^{\circ} \implies \angle{BFD}=\angle{BDF}=72^{\circ} $

$\implies BD=BF=AC=A'C=CF \implies \angle{BFC}=\angle{BFD}+\angle{DFA'}+\angle{A'FC}=168^{\circ}\implies \angle{BCF}=6^{\circ} $

$\implies \angle{BCD}=60^{\circ}-30^{\circ}-6^{\circ}=\bbox[5px, border: 1px solid black]{24^{\circ}}$

---

### 12/12/2021

#### Let $a$, $b$ and $n$ be positive integers such that $n \ge 2$ and $(ab)^{n-1}+1$ divides $a^n+b^n$. Show that $\dfrac{a^n+b^n}{ab^{n-1}+1}$ is a perfect $n^{th}$ power of an integer. i.e., $k=\dfrac{a^n+b^n}{(ab)^{n-1}+1} \in \mathbb{N} \implies \exists c \in \mathbb{N}, k=c^n$. (special case when $n=2$: 1988 IMO Problem 6)

**Prove:**

(1) When $a=b$:

$k=\dfrac{2a^n}{a^{2n-2}+1} \in \mathbb{N} \implies 2a^n=ka^{2n-2}+k \implies 2=ka^{n-2}+\dfrac{k}{a^n}$

$n\ge2, n \in \mathbb{N}, a \in \mathbb{N}, k \in \mathbb{N} \implies n-2 \ge 1 \implies a^{n-2} \ge 1 \implies ka^{n-2} \ge 1 $

$\implies ka^{n-2}=1, \dfrac{k}{a^n}=1 \implies a^{2n-2}=1 \implies a=b=1, k=1$

(2) When $a \ne b$, **WLOG**, suppose $a \gt b$

    (a) When $n=2$

Suppose $k$ is a non-square positive integer and there exist positive integers $(a, b)$ so that $k=\dfrac{a^2+b^2}{ab+1}$. Among these positive integers, suppose $(A, B)$ are the ones satisfying $k=\dfrac{A^2+B^2}{AB+1}$ and such that $A+B$ is minimized, and WLOG, assume $A \gt B$.

Fixing $B$, then $A$ is one root $x_1=A$ of equation $x^2-(kB)x + (B^2-k)=0$. Then we know the other root $x_2$ satisfies $x_2=kB-A$ and $x_2=\dfrac{B^2-k}{A}$.

$x_2=kB-A \implies x_2 \in \mathbb{Z}$. $k$ is not a perfect square and $x_2=\dfrac{B^2-k}{A} \implies x_2 \ne 0$

$\dfrac{x_2^2+B^2}{x_2B+1}=k \gt 0 \implies x_2 \gt 0 \implies x_2 \in \mathbb{N}$

$A \gt B \implies A^2 \gt B^2 \gt B^2-k \implies A \gt \dfrac{B^2-k}{A} \implies  x_2=\dfrac{B^2-k}{A} \lt x_1 = A \implies x_2 + B \lt A + B$

This means, with $B$ fixed, we have $x_2$ as a smaller root than $x_1=A$ and we get even smaller $x_2+B \lt A+B$. This contradicts the minimality of $A+B$.

This means $x_2$ can be smaller and smaller until it reaches $0$ and that means $k=B^2$. The original assumption is not correct and $k$ is a perfect square.

    (b) When $n \gt 2$

We have $n \gt 2, a \gt b, k=\dfrac{a^n+b^n}{(ab)^{n-1}+1}, a,b,k,n \in \mathbb{N} \implies b^n-k=(kb^{n-1}-a)a^{n-1}$

        (1) If $k > b^n$, then $k>k-b^n=a^{n-1}(a-kb^{n-1}) >0 \implies a-kb^{n-1}>0 \implies a-kb^{n-1} \ge 1 \implies k \ge a^{n-1} \implies a>kb^{n-1}\ge k \ge a^{n-1} \implies a > a^{n-1}$ this is not possible

        (2) If $k < b^n$, and since $b<a$ then $kb^{n-1}-a=\dfrac{b^n-k}{a^{n-1}} < \dfrac{b^n}{a^{n-1}} < \dfrac{b^n}{b^{n-1}}=b \implies kb^{n-1}<a+b \implies (k-1)b^{n-1}<a+b-b^{n-1} \le a \implies (k-1)b^{n-1} < a$

and $k<b^n \implies b^n-k=(kb^{n-1}-a)a^{n-1} > 0 \implies kb^{n-1}-a > 0 \implies kb^{n-1}-a \ge 1$

if $k > 1$, then $2 \le k \implies 1 \le k-1 \implies b^{n-1} \le (k-1)b^{n-1} < a \implies b^{n-1}<a \implies b^n-k=(kb^{n-1}-a)a^{n-1} \ge a^{n-1} > (b^{n-1})^{n-1} \ge b^n \implies b^n-k > b^n$ this is not possible, so the only possible situation is $k=1=1^n$ , then the statement is proved true for this case.

        (3) If $k=b^n$ then the statement is proved true for this case as well.

**References:**

* The case $n=2$ of this problem is mentioned in [Vieta Jumping Wiki](https://en.wikipedia.org/wiki/Vieta_jumping)
* The case $n=2$ of this problem is mentioned in book **Problem-Solving Strategies** by **Arthur Engel**, in Chapter 6, E15.
* The case $n=2$ of this problem is also mentioned in book **Modern Olympiad Number Theory** by **Aditya Khurmi**, in Chapter 4, Example 4.7.1.

* [Alternative proof that $(a^2+b^2)/(ab+1)$ is a square when it's an integer](https://math.stackexchange.com/questions/28438/alternative-proof-that-a2b2-ab1-is-a-square-when-its-an-integer)
* [When is $f(a,b)=\dfrac{a^2+b^2}{1+ab}$ a perfect square rational number?](https://mathoverflow.net/questions/250172/when-is-fa-b-fraca2b21ab-a-perfect-square-rational-number/250187#250187)
* [AOPS link 1](https://artofproblemsolving.com/community/c6h57282)
* [AOPS link 2](https://artofproblemsolving.com/community/c146h150371)
* [AOPS link 3](https://artofproblemsolving.com/community/c6h349211)
* [What is the algebraic intuition behind Vieta jumping in IMO1988 Problem 6?](https://math.stackexchange.com/questions/1897942/what-is-the-algebraic-intuition-behind-vieta-jumping-in-imo1988-problem-6)
* [Underlying structure behind the infamous IMO 1988 Problem 6](https://mathoverflow.net/questions/289572/underlying-structure-behind-the-infamous-imo-1988-problem-6)
* [When do Pell equation results imply applicability of the "Vieta jumping"-method to a given conic?](https://math.stackexchange.com/questions/38528/when-do-pell-equation-results-imply-applicability-of-the-vieta-jumping-method)
* [The Legend of Question Six - Numberphile](https://youtu.be/Y30VF3cSIYQ)

---

