---
title: April 2021 Monthly Problems
date: 2021-04-01 11:35
category:
author:
tags: []
summary:
---

### 04/01/2021

#### In $\triangle{ABC}, \angle{ABC}=30^{\circ}, \angle{ACB}=40^{\circ}$, $D$ is on $BC$ so that $AC=BD$, Find $\angle{DAC}$.

![image-20210401181027786](/assets/images/2021-04/image-20210401181027786.png){:class="image--x2l"}

**Solve:**

![image-20210401182009292](/assets/images/2021-04/image-20210401181410006.png){:class="image--x2l"}

Make the circum-circle of $\triangle{ABC}$ and let its center to be $O$.

$\angle{ABC}=30^{\circ} \implies \angle{AOC}=60^{\circ}, AC=OC \implies \angle{OCB}=20^{\circ}$

$BO=CO \implies \angle{OBC}=20^{\circ}, BD=AC=CO=BO$

Connect $DO$, easy to see that $\angle{BOD}=\angle{BDO}=80^{\circ}$

$\angle{DOC}=180^{\circ}-\angle{OBC}-\angle{OCB}-\angle{BOD}$

$=180^{\circ}-20^{\circ}-20^{\circ}-80^{\circ}=60^{\circ}=\angle{AOC}$

$\implies O, D, A$ collinear $\implies \angle{DAC}=\angle{OAC}=\boxed{60^{\circ}}$

---

### 04/02/2021

#### In $\triangle{ABC}, \angle{ABC}=40^{\circ}, \angle{BAC}=80^{\circ}, \angle{ACB}=60^{\circ}$, $I$ is the in-center. Prove:

#### (1) $BI=AC; $  (2) $CD+AD=AC+AE;$  (3) $2AC=CD+AB$

![image-20210402020530225](/assets/images/2021-04/image-20210402020530225.png){:class="image--x2l"}

**Prove:**

(1) Let $D$ be the center of circumcircle of $\triangle{BIC} \implies OB=OI=OC$

![image-20210402020808023](/assets/images/2021-04/image-20210402020808023.png){:class="image--x2l"}

$\angle{BCI}=30^{\circ} \implies \angle{BOI}=60^{\circ} \implies \triangle{BOI} $ is equilateral

$\implies \angle{OBI}=60^{\circ} \implies \angle{OBC}=40^{\circ} \implies \angle{OCB}=40^{\circ}$

$\implies \angle{OCI}=70^{\circ} \implies \angle{COI}=180^{\circ}-2*\angle{OCI}=40^{\circ}$

$\implies \angle{COI}+\angle{OCB}+\angle{ACB}+\angle{CAI}=40^{\circ}+40^{\circ}+60^{\circ}+40^{\circ}=180^{\circ}$

$\implies A, I, O $ is collinear $\implies \angle{COA}=\angle{OAC}=40^{\circ} \implies AC=CO=BI \blacksquare$

(2) Easy to know from (1) that $\angle{AEI}=\angle{AIE}=70^{\circ} \implies AE=AI$

Also $\angle{AOC}=\angle{BCO}=40^{\circ} \implies CD=OD$

So $AD+DC=AD+DO=AO=AI+OI=AE+AC\blacksquare$

![image-20210402143535372](/assets/images/2021-04/image-20210402143535372.png){:class="image--x2l"}

(3) Let $I$ be on $AE$ so that $\angle{AIH}=40^{\circ} \implies AH=HI$

$\angle{AIE}=70^{\circ} \implies \angle{HIE}=30^{\circ}$

$\implies \angle{AHI}=80^{\circ}=\angle{BIH}=\angle{BIE}+\angle{HIE}=80^{\circ}$

$\implies BH=BI \implies AB=BI+DI $

$\implies AC=AB-DI $

$\implies 2AC=AC-DI+AB=OI-DI+AB=OD+AB=CD+AB\blacksquare$

![image-20210402144926276](/assets/images/2021-04/image-20210402144926276.png){:class="image--x2l"}

---

### 04/02/2021

#### In $\triangle{ABC}, \angle{ABC}=15^{\circ}, ACB=30^{\circ},$ $D$ is midpoint of $BC$. Find $\angle{DAB}$.

![image-20210402151152579](/assets/images/2021-04/image-20210402151152579.png){:class="image--x3l"}

**Solve:**

![image-20210402151917804](/assets/images/2021-04/image-20210402151917804.png){:class="image--x3l"}

Extend $CA$ to $O$ so that $\angle{AOD}=30^{\circ} \implies CD=OD=DB$

And $\angle{ODB}=60^{\circ} \implies \triangle{ODB}$ is equilateral

$\implies \angle{DBO}=\angle{DOB}=60^{\circ} \implies \angle{ABO}=45^{\circ}, \angle{AOB}=90^{\circ}$

$\implies \angle{OAB}=180^{\circ}-90^{\circ}-45^{\circ}=45^{\circ} \implies \angle{OAB}=\angle{ABO}$

$\implies AO=BO=DO \implies \angle{DAO}=75^{\circ}$

$\implies \angle{DAB}=75^{\circ}-45^{\circ}=\boxed{30^{\circ}}$

---

### 04/05/2021

#### Let $ABC$ be a triangle and $X$ an interior point of $\triangle{ABC}$. Show that at least one of the angles $\angle{XAB}, \angle{XBC}, \angle{XCA}$ is less than or equal to $30^{\circ}$. **IMO 1991 B2**

**Prove:**

Prove by contradiction: if none of the angles $\angle{XAB}, \angle{XBC}, \angle{XCA}$ is less than or equal to $30^{\circ}$, then

$\angle{XAB} + \angle{XBC} + \angle{XCA} > 90^{\circ}$
$\implies \angle{XAC} + \angle{XCB} + \angle{XBA} < 90^{\circ}$

$sin(\angle{XAB}) > \dfrac{1}{2}, sin(\angle{XBC}) > \dfrac{1}{2}, sin(\angle{XCA}) > \dfrac{1}{2}$
$\implies sin(\angle{XAB}) \cdot sin(\angle{XBC}) \cdot sin(\angle{XCA}) > \dfrac{1}{8}$

From [Trigonometric Form of Ceva's Theorem](https://www.cut-the-knot.org/triangle/TrigCeva.shtml) we know

$sin(\angle{XAB}) \cdot sin(\angle{XBC}) \cdot sin(\angle{XCA}) = sin(\angle{XAC}) \cdot sin(\angle{XCB}) \cdot sin(\angle{XBA})$
$\implies sin(\angle{XAC}) \cdot sin(\angle{XCB}) \cdot sin(\angle{XBA}) > \dfrac{1}{8}$
where $\angle{XAC} + \angle{XCB} + \angle{XBA} < 90^{\circ}$

Let $x=\angle{XAC}, y=\angle{XCB}, z=\angle{XAC}$

$\implies 0 < z < 90^{\circ} - x - y$

$\implies 0 < sin(z) < sin(90^{\circ} - x - y) = cos(x + y) $

$\implies sin(x) \cdot sin(y) \cdot cos(x + y) > sin(x) \cdot sin(y) \cdot sin(z) > \dfrac{1}{8}$

where $0 < x + y < 90^{\circ}$

$\implies \dfrac{1}{2}(cos(x-y) - cos(x+y))cos(x + y) > \dfrac{1}{8}$

$\implies 4(cos(x-y) - cos(x+y))cos(x + y) > 1$

Obviously $ 1 \ge cos(x-y)$

$\implies 4(1 - cos(x + y))cos(x + y) \ge 4(cos(x - y)-cos(x+y))cos(x + y) > 1$

$\implies 4(cos(x + y) - 1)cos(x + y) +1 < 0$

$\implies (2cos(x+ y)-1)^2 < 0$

This is impossible. So we know the assumption is not correct. $\blacksquare$

Above analysis means that, for $sin(x)sin(y)cos(x+y), 0 < x + y < \dfrac{\pi}{2}$, it gets maximum value when $cos(x-y)=0 \implies x=y$ and $ (2cos(x+y) - 1)^2=0 \implies cos(x+y)=\dfrac{1}{2} \implies x=y=\dfrac{\pi}{6}$

We can verify this by [Wolfram](https://www.wolframalpha.com/input/?i=findmaximum%5Bsin%28x%29*sin%28y%29*cos%28x%2By%29%2C+0%3Cx%2By%3Cpi%2F2%5D):

$ max \bigg \\{ sin(x)sin(y)cos(x+y) \bigg \| 0< x+y < \dfrac{\pi}{2} \bigg \\} = 0.125 \text{ at } (x,y) \approx (0.523599, 0.523599) $

---

### 04/18/2021

#### Solve $\sqrt{x-\dfrac{1}{x}}+\sqrt{1-\dfrac{1}{x}}=x$

**Solve:**

$\sqrt{x-\dfrac{1}{x}}-\sqrt{1-\dfrac{1}{x}} = \dfrac{x-\dfrac{1}{x}-1+\dfrac{1}{x}}{\sqrt{x-\dfrac{1}{x}}+\sqrt{1-\dfrac{1}{x}}} = \dfrac{x-1}{x}$
$\implies 2\sqrt{x-\dfrac{1}{x}}=x-\dfrac{1}{x}+1$

Let $x-\dfrac{1}{x}=y \implies 2y=y^2+1 \implies y=1 \implies x-\dfrac{1}{x}=1$
$\implies x^2-x-1=0 \implies x=\dfrac{1\pm\sqrt{5}}{2}$

But $x \ge 0 \implies x=\boxed{\dfrac{1+\sqrt{5}}{2}}$

---
