---
title: October 2021
date: 2021-10-12 14:58
tags: []
marp: true
---

### 10/21/2021

#### $$\angle{B}=80^{\circ}$$ in $$\triangle{ABC}$$ and $$BD$$ is angle bisector which makes $$AD=BC+BD$$. Find $$\angle{A}$$.

![image-20211104144756045](/assets/images/2021/image-20211104144756045.png)

**Solve 1:**

![image-20211106061924939](/assets/images/2021/image-20211106061924939.png)

(Chinese Version: )

$$AD=BC+BD \gt BD \implies \angle{A} < \angle{ABD} \implies \angle{A} \lt 40^{\circ}$$。令 $$\angle{A}=\alpha \in (0， 40^{\circ})$$。

$$\dfrac{AD}{BD}=\dfrac{sin(40^{\circ})}{sin(\alpha)}=\dfrac{BC+BD}{BD}=1+\dfrac{BC}{BD}=1+\dfrac{sin(\angle{BDC})}{sin(\angle{C})}=1+\dfrac{sin(\alpha+40^{\circ})}{sin(\alpha+80^{\circ})}$$

$$=\dfrac{sin(\alpha+80^{\circ})+sin(\alpha+40^{\circ})}{sin(\alpha+80^{\circ})}=\dfrac{2sin(\alpha+60^{\circ})cos(20^{\circ})}{sin(\alpha+80^{\circ})} \implies sin(\alpha)sin(\alpha+60^{\circ})=sin(\alpha+80^{\circ})sin(20^{\circ})$$

令$$f(\alpha)=sin(\alpha)sin(\alpha+60^{\circ})-sin(\alpha+80^{\circ})sin(20^{\circ})$$, 显见 $$f(20^{\circ})=0$$ 且

$$f'(\alpha)=cos(\alpha)sin(\alpha+60^{\circ})+sin(\alpha)cos(\alpha+60^{\circ})-sin(20^{\circ})cos(\alpha+80^{\circ})=sin(2\alpha+60^{\circ})-sin(20^{\circ})cos(\alpha+80^{\circ})$$

$$\alpha \in (0， 40^{\circ}) \implies sin(2\alpha+60^{\circ}) \gt sin(40^{\circ}) \gt sin(20^{\circ})cos(\alpha+80^{\circ}) \implies f '(\alpha) \gt 0 \implies \angle{A}=\bbox[1px, border: 1px solid black]{20^{\circ}}$$为唯一解。

(English Verison: )

$$AD=BC+BD \gt BD \implies \angle{A} < \angle{ABD} \implies \angle{A} \lt 40^{\circ}$$. Let $$\angle{A}=\alpha \in (0， 40^{\circ})$$。

$$\dfrac{AD}{BD}=\dfrac{sin(40^{\circ})}{sin(\alpha)}=\dfrac{BC+BD}{BD}=1+\dfrac{BC}{BD}=1+\dfrac{sin(\angle{BDC})}{sin(\angle{C})}=1+\dfrac{sin(\alpha+40^{\circ})}{sin(\alpha+80^{\circ})}$$

$$=\dfrac{sin(\alpha+80^{\circ})+sin(\alpha+40^{\circ})}{sin(\alpha+80^{\circ})}=\dfrac{2sin(\alpha+60^{\circ})cos(20^{\circ})}{sin(\alpha+80^{\circ})} \implies sin(\alpha)sin(\alpha+60^{\circ})=sin(\alpha+80^{\circ})sin(20^{\circ})$$

Let $$f(\alpha)=sin(\alpha)sin(\alpha+60^{\circ})-sin(\alpha+80^{\circ})sin(20^{\circ})$$, obviously $$f(20^{\circ})=0$$ and

$$f'(\alpha)=cos(\alpha)sin(\alpha+60^{\circ})+sin(\alpha)cos(\alpha+60^{\circ})-sin(20^{\circ})cos(\alpha+80^{\circ})=sin(2\alpha+60^{\circ})-sin(20^{\circ})cos(\alpha+80^{\circ})$$

$$\alpha \in (0， 40^{\circ}) \implies sin(2\alpha+60^{\circ}) \gt sin(40^{\circ}) \gt sin(20^{\circ})cos(\alpha+80^{\circ}) \implies f '(\alpha) \gt 0 \implies \angle{A}=\bbox[1px, border: 1px solid black]{20^{\circ}}$$ is the only solution.



**Solve 2:**

![image-20211105171659093](/assets/images/2021/image-20211105165800293.png)

(Chinese Version):

$$AB$$上取$$E$$使得$$DE \parallel BC$$, $$BC$$上取$$G$$使得$$DG \parallel AB$$, $$AD$$上取$$F$$使得$$\angle{EFD}=40^{\circ}$$。

$$DE \parallel BC, DG \parallel AB \implies \angle{EDB}=\angle{CBD}=40^{\circ}=\angle{DBE}=\angle{BDG} \implies BE=DE=DG$$

$$DE \parallel BC \implies \angle{FDE}=\angle{DCB}$$, 且 $$\angle{CBD}=\angle{EFD}=40^{\circ} \implies \triangle{DEF} \sim \triangle{CDB}$$

比较 $$CD$$ 与 $$BE$$. 共三种可能性：

1) 假设 $$CD=BE \implies CD=DG \implies \angle{C}=\angle{DGC}=\angle{EBC}=80^{\circ}\implies \angle{A}=20^{\circ}$$
2) 假设 $$CD \gt BE \implies CD \gt DG \implies \angle{C} < \angle{DGC} \implies \angle{C} \lt 80^{\circ} \implies \angle{A} \gt 20^{\circ}$$
   由于$$\angle{A}+\angle{AEF}=40^{\circ} \implies \angle{A}>\angle{AEF} \implies EF \gt AF$$
   $$CD\gt BE \implies CD \gt DE$$, 由于$$\triangle{DEF} \sim \triangle{CDB}$$, 易知 $$BD \gt EF, BC \gt DF$$
   $$BC \gt DF, AD=DF+AF=BC+BD \implies BD \lt AF \implies BD \lt EF$$
   这样同时有 $$BD \lt EF$$ 以及 $$BD \gt EF$$ 矛盾，所以 $$CD \gt BE$$ 的假设不真。
3) 假设 $$CD < BE$$, 类似可知同样会推出矛盾，所以 $$CD \lt BE$$ 的假设不真。

从而只能 $$CD=BE \implies \angle{C}=80^{\circ} \implies \angle{A}=\bbox[1px, border: 1px solid black]{20^{\circ}}$$.

(English Version):

Let $$E$$ on side $$AB$$ and $$DE \parallel BC$$. Let $$G$$ on side $$BC$$ and $$DG \parallel AB. $$ Let $$F$$ on side $$AC$$ and $$\angle{EFD}=40^{\circ}$$.

$$DE \parallel BC, DG \parallel AB \implies \angle{EDB}=\angle{CBD}=40^{\circ}=\angle{DBE}=\angle{BDG} \implies BE=DE=DG$$

$$DE \parallel BC \implies \angle{FDE}=\angle{DCB}$$, and we have $$\angle{CBD}=\angle{EFD}=40^{\circ} \implies \triangle{DEF} \sim \triangle{CDB}$$

Compare $$CD$$ and $$BE$$. There are three possibilities:

1) If $$CD=BE \implies CD=DG \implies \angle{C}=\angle{DGC}=\angle{EBC}=80^{\circ}\implies \angle{A}=20^{\circ}$$
2) If $$CD \gt BE \implies CD \gt DG \implies \angle{C} < \angle{DGC} \implies \angle{C} \lt 80^{\circ} \implies \angle{A} \gt 20^{\circ}$$
   Since $$\angle{A}+\angle{AEF}=40^{\circ} \implies \angle{A}>\angle{AEF} \implies EF \gt AF$$
   $$CD\gt BE \implies CD \gt DE$$, since $$\triangle{DEF} \sim \triangle{CDB}$$, we know $$BD \gt EF, BC \gt DF$$
   $$BC \gt DF, AD=DF+AF=BC+BD \implies BD \lt AF \implies BD \lt EF$$
   Thus we have $$BD \lt EF$$ and $$BD \gt EF$$ as contradiction, so we know $$CD > BE$$ is false.
3) If $$CD < BE$$, by similar deduction we can know this is false as well.

Then we know $$CD=BE \implies \angle{C}=80^{\circ} \implies \angle{A}=\bbox[1px, border: 1px solid black]{20^{\circ}}$$.

**Solve 3 (via trigonometry):**

From the Laws of Sines we know that

![image-20211104150631700](/assets/images/2021/image-20211104145243160.png)

$$\dfrac{AD}{sin(40^{\circ})}=\dfrac{AB}{sin(40^{\circ}+x)} \implies AD=\dfrac{sin(40^{\circ})}{sin(40^{\circ}+x)}AB,$$

$$\dfrac{BD}{sin(x)}=\dfrac{AB}{sin(40^{\circ}+x)} \implies BD=\dfrac{sin(x)}{sin(40^{\circ}+x)}AB, $$

$$\dfrac{BC}{sin(x)}=\dfrac{AB}{sin(80^{\circ}+x)} \implies BC=\dfrac{sin(x)}{sin(80^{\circ}+x)}AB$$

$$AD=BC+BD \implies \dfrac{sin(40^{\circ})}{sin(40^{\circ}+x)}=\dfrac{sin(x)}{sin(40^{\circ}+x)}+\dfrac{sin(x)}{sin(80^{\circ}+x)}$$

$$\implies sin(40^{\circ})sin(80^{\circ}+x)-sin(x)sin(80^{\circ}+x)=sin(x)sin(40^{\circ}+x)$$

Use $$sin(A)sin(B)=-\dfrac{1}{2}(cos(A+B)-cos(A-B))$$, we get $$[cos(120^{\circ}+x)-cos(40^{\circ}+x)]-[cos(80^{\circ}+2x)-cos(80^{\circ})]=cos(40^{\circ}+2x)-cos(40^{\circ})$$

$$\implies cos(80^{\circ}+2x)-cos(80^{\circ})+cos(60^{\circ}-x)+cos(40^{\circ}+x)=cos(40^{\circ})-cos(40^{\circ}+2x)$$

$$\implies cos(80^{\circ}+2x)+cos(40^{\circ}+2x)+cos(60^{\circ}-x)+cos(40^{\circ}+x)=cos(40^{\circ})+cos(80^{\circ})$$

Use $$cos(A)+cos(B)=2cos(\dfrac{A+B}{2})cos(\dfrac{A-B}{2})$$, we get

$$2cos(60^{\circ}+2x)cos(20^{\circ})+2cos(50^{\circ})cos(10^{\circ}-x)=2cos(60^{\circ})cos(20^{\circ})$$

$$\implies cos(50^{\circ})cos(10^{\circ}-x)=cos(20^{\circ})[cos(60^{\circ})-cos(60^{\circ}+2x)]$$

Use $$cos(A)-cos(B)=-2sin(\dfrac{A+B}{2})sin(\dfrac{A-B}{2})$$, we get

$$cos(50^{\circ})cos(10^{\circ}-x)=2cos(20^{\circ})sin(60^{\circ}+x)sin(x)$$

$$\implies sin(40^{\circ})sin(80^{\circ}+x)=2sin(20^{\circ})cos(20^{\circ})sin(100^{\circ}-x)=2cos(20^{\circ})sin(60^{\circ}+x)sin(x)$$

$$\implies sin(20^{\circ})sin(100^{\circ}-x)=sin(60^{\circ}+x)sin(x)$$

By observation, $$x=20^{\circ}$$. This is from original approach. Not strict step here.

**Unsolved Approach:**

![image-20211104150631700](/assets/images/2021/image-20211104145243160.png)

Let $$BC=a, AB=d, CD=c, BD=b$$, then $$AD=a+b$$

- $$\dfrac{a}{c}=\dfrac{d}{a+b} \implies d=\dfrac{a(a+b)}{c} \implies ad=\dfrac{a^2(a+b)}{c}, a+d=\dfrac{a(a+b+c)}{c}$$

And we know from the length of angle sector that $$b^2=ad-\dfrac{(a+b+c)^2ad}{(a+d)^2}=\dfrac{a^2(a+b)}{c}-\dfrac{(a+b+c)^2\dfrac{a^2(a+b)}{c}}{\dfrac{a^2(a+b+c)^2}{c^2}}=\dfrac{a^2(a+b)}{c}-c(a+b)=\dfrac{(a^2-c^2)(a+b)}{c}$$

$$\implies cos(\angle{BDC})=\dfrac{b^2+c^2-a^2}{2bc}=\dfrac{c^2-a^2+\dfrac{(a^2-c^2)(a+b)}{c}}{2bc}=\dfrac{(a^2-c^2)(a+b-c)}{2bc^2}$$



From Laws of Sines we know $$\dfrac{d}{sin(\angle{C})}=\dfrac{a+b+c}{sin80^{\circ}} \implies \dfrac{a(a+b)}{csin(\angle{C})}=\dfrac{a+b+C}{sin80^{\circ}} \implies sin(\angle{C})=\dfrac{a(a+b)sin80^{\circ}}{c(a+b+c)}$$

and we also know $$\dfrac{b}{sin(\angle{C})}=\dfrac{c}{sin40^{\circ}}\implies \dfrac{bc(a+b+c)}{a(a+b)sin80^{\circ}}=\dfrac{c}{sin40^{\circ}} \implies \dfrac{b(a+b+c)}{2a(a+b)sin40^{\circ}cos40^{\circ}}=\dfrac{1}{sin40^{\circ}}$$

$$\implies cos40^{\circ}=\dfrac{b(a+b+c)}{2a(a+b)}=\dfrac{a^2+b^2-c^2}{2ab} \implies \dfrac{b^2(a+b+c)}{a+b}=a^2+b^2-c^2 \implies b^2+\dfrac{b^2c}{a+b}=a^2+b^2-c^2$$

$$\implies a^2-c^2=\dfrac{b^2c}{a+b} \implies cos(\angle{BDC})=\dfrac{(a^2-c^2)(a+b-c)}{2bc^2} = \dfrac{\dfrac{b^2c}{a+b}(a+b-c)}{2bc^2}=\dfrac{b(a+b-c)}{2c(a+b)}=\dfrac{b-\dfrac{bc}{a+b}}{2c}$$

if $$cos(\angle{BDC})=\dfrac{1}{2} \implies b-c=\dfrac{bc}{a+b}$$

---

### 10/22/2021

#### How many distinct permutations from $$1,1,2,2,3,3,4,4$$ that there are no equal consecutive numbers?

**Solve:**

1. Calculate all distinct permutations of $$1,1,2,2,3,3,4,4$$. The generate function for all distinct permutations of $$1,1,2,2,3,3,4,4$$ is $$g(x)=(1+x+\dfrac{x^2}{2!})^4$$ , its coefficient of $$x^8$$ in $$g(x)$$ is $$\dfrac{1}{16}$$, so the number of total distinct permutations is $$\dfrac{1}{16}*8!=2520$$.

2. Calculate all distinct permutations of $$1,1,2,2,3,3,4,4$$ that contains $$1$$ pair of equal consecutive numbers. There are $$4 \choose 1$$ ways to choose the equal consecutive number, and take it as one number to permute with other $$6$$ numbers, so the generate function is $$(1+x)(1+x+\dfrac{x^2}{2!})^3$$, its coefficient of $$x^7$$ is $$\dfrac{1}{8}$$, so the number of distinct permutations is $$4 * \dfrac{1}{8} * 7! = 2520$$.

3. Calculate all distinct permutations of $$1,1,2,2,3,3,4,4$$ that contains $$2$$ pairs of equal consecutive numbers. There are $$4 \choose 2$$ ways to choose the equal consecutive numbers and take each of them as one number to permute with other 4 numbers, so the generate function is $$(1+x)^2(1+x+\dfrac{x^2}{2})^2$$, its coefficient of $$x^6$$ is $$\dfrac{1}{4}$$, so the number of distinct permutations is $${4 \choose 2} * \dfrac{1}{4} * 6!=1080$$.

4. Calculate all distinct permutations of $$1,1,2,2,3,3,4,4$$ that contains $$3$$ pairs of equal consecutive numbers. There are $$4 \choose 3$$ ways to choose the equal consecutive numbers and take each of them as one number to permute with the rest 2 numbers, so the generate function is $$(1+x)^3(1+x+\dfrac{x^2}{2})$$, its coefficient of $$x^5$$ is $$\dfrac{1}{2}$$, so the number of distinct permutations is $${4 \choose 3} * \dfrac{1}{2} * 5!=240$$.

5. Calculate all distinct permutations of $$1,1,2,2,3,3,4,4$$ that contains $$4$$ pairs of equal consecutive numbers. Take each of pair of them as one number, so this is permutation of 4 numbers: $$4!=24$$.

   According to PIE, the result is $$2520-2520+1080-240+24=\bbox[1px, border: 1px solid black]{864}$$.

---









