---
title: Jan 2022 Problems
date: 2022-01-03 05:24
tags: []
---

### 01/16/2022

#### $I$ is the incenter of $\triangle{ABC}$ and $D$ is the tangent point of the incircle with side $BC$. Points $E$ and $F$ are on side $BC$ so that $\angle{BAE}=\angle{ACB}, \angle{CAF}=\angle{ABC}$. $G$ and $H$ are incenters of $\triangle{ABE}$ and $\triangle{ACF}$ respectively. Prove that $AD$ is the Euler Line of $\triangle{GHI}$.

![image-20211230201638718](/assets/images/2021-12/image-20211230201638718.png)

**Prove:**

Let $s=\dfrac{a+b+c}{2}, S_A=\dfrac{b^2+c^2-a^2}{2}, S_B=\dfrac{c^2+a^2-b^2}{2}, S_C=\dfrac{a^2+b^2-c^2}{2}$

$\overrightarrow{I}=\dfrac{a\overrightarrow{A}+b\overrightarrow{B}+c\overrightarrow{C}}{a+b+c}$

$\overrightarrow{G}=\dfrac{\dfrac{c^2}{a}\overrightarrow{A}+\dfrac{bc}{a}\overrightarrow{B}+c(\dfrac{c^2}{a^2}\overrightarrow{C}+(1-\dfrac{c^2}{a^2})\overrightarrow{B})}{\dfrac{c^2}{a}+\dfrac{bc}{a}+c}=\dfrac{c\overrightarrow{A}+(b+\dfrac{a^2-c^2}{a})\overrightarrow{B}+(\dfrac{c^2}{a})\overrightarrow{C}}{a+b+c}$

$\overrightarrow{H}=\dfrac{\dfrac{b^2}{a}\overrightarrow{A}+b((1-\dfrac{b^2}{a^2})\overrightarrow{C}+\dfrac{b^2}{a^2}\overrightarrow{B})+\dfrac{bc}{a}\overrightarrow{C}}{\dfrac{b^2}{a}+b+\dfrac{bc}{a}}=\dfrac{b\overrightarrow{A}+(\dfrac{b^2}{a})\overrightarrow{B}+(c+\dfrac{a^2-b^2}{a})\overrightarrow{C}}{a+b+c}$

$\overrightarrow{G_{GHI}}=\dfrac{\overrightarrow{G}+\overrightarrow{H}+\overrightarrow{I}}{3}=\dfrac{(a+b+c)\overrightarrow{A}+(2b+\dfrac{a^2+b^2-c^2}{a})\overrightarrow{B}+(2c+\dfrac{a^2+c^2-b^2}{a})\overrightarrow{C}}{a+b+c}$

$=\overrightarrow{A}+\dfrac{(a+b)^2-c^2}{a(a+b+c)}\overrightarrow{B}+\dfrac{(a+c)^2-b^2}{a(a+b+c)}\overrightarrow{C}=\overrightarrow{A}+\dfrac{a+b-c}{a}\overrightarrow{B}+\dfrac{a+c-b}{a}\overrightarrow{C}=\overrightarrow{A}+\dfrac{2s-2c}{a}\overrightarrow{B}+\dfrac{2s-2b}{a}\overrightarrow{C}$

To prove that $AD$ is the Euler Line of $\triangle{GHI}$, check if $\overrightarrow{G_{GHI}}$ is colinear with $\overrightarrow{A}$ and $\overrightarrow{D}=\dfrac{s-c}{a}\overrightarrow{B}+\dfrac{s-b}{a}\overrightarrow{C}$:
$$
\begin{align*}
\begin{vmatrix}
1 & 0 & 0\\
1 & \dfrac{s-c}{a} & \dfrac{s-b}{a}\\
1 & \dfrac{2s-2c}{a} & \dfrac{2s-2b}{a}
\end{vmatrix}&=\dfrac{s-c}{a}\dfrac{2s-2b}{a}-\dfrac{s-b}{a}\dfrac{2s-2c}{a}=0 \implies \overrightarrow{G_{GHI}}, \overrightarrow{A}, \overrightarrow{D} \text{ are collinear}
\end{align*}
$$

Now we prove that the circumcenter of $\triangle{GHI}$ is also collinear with $A,D$:

$cosB=\dfrac{a^2-b^2+c^2}{2ac}, sinB=\dfrac{2S}{ab} \implies x_A=c\cdot cosB=\dfrac{a^2-b^2+c^2}{2a}, y_A=c \cdot sinB=\dfrac{2S}{a}$

Let $A(\dfrac{a^2-b^2+c^2}{2a}, \dfrac{2S}{a}), B(0,0), C(a,0)$, Convert Barycentric Coordinates of point $G,H,I$ to Cartesian Coordinates:

$$
\begin{align*}
\begin{bmatrix}
\overrightarrow{G} & \overrightarrow{H} & \overrightarrow{I}
\end{bmatrix}&=
\begin{bmatrix}
\dfrac{a^2-b^2+c^2}{2a} & 0 & a\\
\dfrac{2S}{a} & 0 & 0\\
1 & 1 & 1
\end{bmatrix}
\begin{bmatrix}
\dfrac{c}{a+b+c} & \dfrac{b}{a+b+c} & \dfrac{a}{a+b+c}\\
\dfrac{b+\dfrac{a^2-c^2}{a}}{a+b+c} & \dfrac{\dfrac{b^2}{a}}{a+b+c} & \dfrac{b}{a+b+c}\\
\dfrac{\dfrac{c^2}{a}}{a+b+c} & \dfrac{c+\dfrac{a^2-b^2}{a}}{a+b+c} & \dfrac{c}{a+b+c}
\end{bmatrix}\\
&=
\begin{bmatrix}
\dfrac{c(a-b+c)}{2a} & \dfrac{2a^2-b(a+b-c)}{2a} & \dfrac{a-b+c}{2} \\
\dfrac{2cS}{a(a+b+c)} & \dfrac{2bS}{a(a+b+c)} & \dfrac{2S}{a+b+c} \\
1 & 1 & 1
\end{bmatrix}
\end{align*}
$$
.

The Wolfram link of above calculation is [here](https://www.wolframalpha.com/input/?i=Simplify+%7B%7B%28a%5E2-b%5E2%2Bc%5E2%29%2F%282a%29%2C+0%2C+a%7D%2C+%7B2S%2Fa%2C+0%2C+0%7D%2C+%7B1%2C+1%2C+1%7D%7D+.+%7B%7Bc%2C+b%2C+a%7D%2C+%7B%28b%2B%28a%5E2-c%5E2%29%2Fa%29%2C+%28b%5E2%2Fa%29%2C+b%7D%2C+%7B%28c%5E2%2Fa%29%2C+%28c%2B%28a%5E2-b%5E2%29%2Fa%29%2C+c%7D%7D++%2F%28a%2Bb%2Bc%29). Now we know that

$AB=c, AC=b, BC=a, BE=\dfrac{c^2}{a}, AE=AF=\dfrac{bc}{a}, CF=\dfrac{b^2}{a} \implies E(\dfrac{c^2}{a}, 0), F(\dfrac{a^2-b^2}{a}, 0)$

$x_G=X_{O_{\triangle{ABE}}}=\dfrac{BE\cdot x_A+AB \cdot x_E+AE \cdot x_B}{BE+AB+AE}=\dfrac{\dfrac{a^2-b^2+c^2}{2a}\dfrac{c^2}{a}+c\dfrac{c^2}{a}}{\dfrac{c^2}{a}+c+\dfrac{bc}{a}}=\dfrac{c(a-b+c)}{2a}$, link [here](https://www.wolframalpha.com/input/?i=Simplify+%5Cdfrac%7B%5Cdfrac%7Ba%5E2-b%5E2%2Bc%5E2%7D%7B2a%7D%5Cdfrac%7Bc%5E2%7D%7Ba%7D%2Bc%5Cdfrac%7Bc%5E2%7D%7Ba%7D%7D%7B%5Cdfrac%7Bc%5E2%7D%7Ba%7D%2Bc%2B%5Cdfrac%7Bbc%7D%7Ba%7D%7D)

$y_G=Y_{O_{\triangle{ABE}}}=\dfrac{BE\cdot y_A+AB \cdot y_E+AE \cdot y_B}{BE+AB+AE}=\dfrac{\dfrac{2S}{a}\dfrac{c^2}{a}}{\dfrac{c^2}{a}+c+\dfrac{bc}{a}}=\dfrac{2cS}{a(a+b+c)}$, link [here](https://www.wolframalpha.com/input/?i=Simplify+%5Cdfrac%7B%5Cdfrac%7B2S%7D%7Ba%7D%5Cdfrac%7Bc%5E2%7D%7Ba%7D%7D%7B%5Cdfrac%7Bc%5E2%7D%7Ba%7D%2Bc%2B%5Cdfrac%7Bbc%7D%7Ba%7D%7D%7D)

$x_H=X_{O_{\triangle{ACF}}}=\dfrac{AF \cdot x_C + FC \cdot x_A + CA \cdot x_F}{AF+FC+CA}=\dfrac{\dfrac{bc}{a}a+b\dfrac{a^2-b^2}{a}+\dfrac{b^2}{a}\dfrac{a^2-b^2+c^2}{2a}}{\dfrac{bc}{a}+\dfrac{b^2}{a}+b}=\dfrac{2a^2-ab-b^2+bc}{2a}$, link [here](https://www.wolframalpha.com/input/?i=Simplify+%5Cdfrac%7B%5Cdfrac%7Bbc%7D%7Ba%7Da%2Bb%5Cdfrac%7Ba%5E2-b%5E2%7D%7Ba%7D%2B%5Cdfrac%7Bb%5E2%7D%7Ba%7D%5Cdfrac%7Ba%5E2-b%5E2%2Bc%5E2%7D%7B2a%7D%7D%7B%5Cdfrac%7Bbc%7D%7Ba%7D%2B%5Cdfrac%7Bb%5E2%7D%7Ba%7D%2Bb%7D)

$y_H=Y_{O_{\triangle{ACF}}}=\dfrac{AF \cdot y_C + FC \cdot y_A + CA \cdot y_F}{AF+FC+CA}=\dfrac{\dfrac{b^2}{a}\dfrac{2S}{a}}{\dfrac{bc}{a}+\dfrac{b^2}{a}+b}=\dfrac{2bS}{a(a+b+c)}$, link [here](https://www.wolframalpha.com/input/?i=Simplify+%5Cdfrac%7B%5Cdfrac%7Bb%5E2%7D%7Ba%7D%5Cdfrac%7B2S%7D%7Ba%7D%7D%7B%5Cdfrac%7Bbc%7D%7Ba%7D%2B%5Cdfrac%7Bb%5E2%7D%7Ba%7D%2Bb%7D)

$x_I=X_{O_{\triangle{ABC}}}=\dfrac{BC \cdot x_A+AB \cdot x_C}{a+b+c}=\dfrac{\dfrac{a^2-b^2+c^2}{2a}a+ac}{a+b+c}=\dfrac{a-b+c}{2}$

$y_I=X_{O_{\triangle{ABC}}}=\dfrac{BC \cdot y_A}{a+b+c}=\dfrac{\dfrac{2S}{a}a}{a+b+c}=\dfrac{2S}{a+b+c}$

From [Circumcenter Wiki](https://en.wikipedia.org/wiki/Circumscribed_circle) we get the formula to calculate the Cartesian Coordinates of circumcemter (See Matlab code below for details):

$$
\begin{align*}
{O_x}&=\dfrac{(x_A^2+y_A^2)(y_B-y_C)+(x_B^2+y_B^2)(y_C-y_A)+(x_C^2+y_C^2)(y_A-y_B)}{2[x_A(y_B-y_C)+x_B(y_C-y_A)+x_C(y_A-y_B)]}
=\dfrac{\begin{vmatrix}x_A^2+y_A^2 & y_A & 1\\ x_B^2+y_B^2 & y_B & 1\\ x_C^2+y_C^2 & y_C & 1\end{vmatrix}}{2\begin{vmatrix}x_A & y_A & 1 \\ x_B & y_B & 1 \\ x_C & y_C & 1\end{vmatrix}} \\ &=\dfrac{a^3+a^2b+a^2c-ab^2+ac^2-b^3+b^2c-bc^2+c^3}{2a(a+b+c)} \\
{O_y}&=\dfrac{(x_A^2+y_A^2)(x_C-x_B)+(x_B^2+y_B^2)(x_A-x_C)+(x_C^2+y_C^2)(x_B-x_A)}{2[x_A(y_B-y_C)+x_B(y_C-y_A)+x_C(y_A-y_B)]}
=\dfrac{\begin{vmatrix}x_A & x_A^2+y_A^2 & 1\\ x_B & x_B^2+y_B^2 & 1\\ x_C & x_C^2+y_C^2 & 1\end{vmatrix}}{2\begin{vmatrix}x_A & y_A & 1 \\ x_B & y_B & 1 \\ x_C & y_C & 1\end{vmatrix}} \\ &=-\dfrac{(a-b+c)(a+b-c)(a^2-b^2-c^2)}{8aS}
\end{align*}
$$.

To prove that $O$ is collinear with $A, D$:

$$
\begin{align*}
\begin{vmatrix}
1 & \dfrac{a-b+c}{2} & 0\\
1 & \dfrac{a^2-b^2+c^2}{2a} & \dfrac{2S}{a}\\
1 & \dfrac{a^3+a^2b+a^2c-ab^2+ac^2-b^3+b^2c-bc^2+c^3}{2a(a+b+c)} & -\dfrac{(a-b+c)(a+b-c)(a^2-b^2-c^2)}{8aS}
\end{vmatrix} = 0
\end{align*}
$$ .

So the points $G_{\triangle{GHI}}$ and $O_{\triangle{GHI}}$ are collinear with $A, D$, this means $AD$ is the Euler Line of $\triangle{GHI} \blacksquare$.

Here is the Matlab code for symbolic calculation:

```matlab
syms a b c s S D a_x a_y b_x b_y c_x c_y o_x o_y_n o_y_d O_X_N O_Y_N O_D o_x_2 o_x_y_2 check_collinear

s = (a + b + c) / 2;
S = sqrt(s * (s - a) * (s - b) * (s - c));
a_x = (a - b + c ) / 2;
a_y = 2 * S / (a + b + c);
b_x = c * (a - b + c) / (2 * a);
b_y = 2 * c * S / (a * (a + b + c));
c_x = (2 * a ^ 2 - a * b - b ^ 2 + b * c) / (2 * a);
c_y = 2 * b * S / (a * (a + b + c));

% Use formular from wiki directly %
D = 2 * (a_x * (b_y - c_y) + b_x * (c_y - a_y) + c_x * (a_y - b_y));
[o_x_n, o_x_d] = numden(((a_x ^ 2 + a_y ^ 2) * (b_y - c_y) + (b_x ^ 2 + b_y ^ 2) * (c_y - a_y) + (c_x ^ 2 + c_y ^ 2) * (a_y - b_y)) / D);
[o_y_n, o_y_d] = numden(((a_x ^ 2 + a_y ^ 2) * (c_x - b_x) + (b_x ^ 2 + b_y ^ 2) * (a_x - c_x) + (c_x ^ 2 + c_y ^ 2) * (b_x - a_x)) / D);

pretty(simplify(o_x_n / o_x_d))
pretty(simplify(o_y_n / o_y_d))
factor(o_x_n)
factor(o_y_n)

% Use determinant approach %
O_X_N = [a_x ^ 2 + a_y ^ 2, a_y, 1; b_x ^ 2 + b_y ^ 2, b_y, 1; c_x ^ 2 + c_y ^ 2, c_y, 1];
O_Y_N = [a_x, a_x ^ 2 + a_y ^ 2, 1; b_x, b_x ^ 2 + b_y ^ 2, 1; c_x, c_x ^ 2 + c_y ^ 2, 1];
O_D = 2 * [a_x, a_y, 1; b_x, b_y, 1; c_x, c_y, 1];

pretty(simplify(det(O_X_N) / det(O_D)))
pretty(simplify(det(O_Y_N) / det(O_D)))

check_collinear = simplify(det([1, (a - b + c) / 2, 0; 1, (a^2 - b^2 + c^2) / (2 * a), (2 * S) / a; 1, o_x_n / o_x_d, o_y_n / o_y_d]));

pretty(check_collinear)
```

And here is the result:

```matlab
>> solved
 3    2      2        2      2    3    2        2    3
a  + a  b + a  c - a b  + a c  - b  + b  c - b c  + c
------------------------------------------------------
                    2 a (a + b + c)

   4      2  2      2          2  2    4      3        2  2        3    4
  a  - 2 a  b  + 2 a  b c - 2 a  c  + b  - 2 b  c + 2 b  c  - 2 b c  + c
- -----------------------------------------------------------------------
         2 a sqrt((a + b + c) (a + b - c) (a - b + c) (b - a + c))


ans =

[-1, a^3 + a^2*b + a^2*c - a*b^2 + a*c^2 - b^3 + b^2*c - b*c^2 + c^3]


ans =

[a - b + c, a + b - c, a^2 - b^2 - c^2]

 3    2      2        2      2    3    2        2    3
a  + a  b + a  c - a b  + a c  - b  + b  c - b c  + c
------------------------------------------------------
                    8 a (a + b + c)

   4           2             4      3               3    4
  a  - #3 + 2 a  b c - #2 + b  - 2 b  c + #1 - 2 b c  + c
- --------------------------------------------------------
                       4              4         4
           8 a sqrt(- a  + #3 + #2 - b  + #1 - c )

where

            2  2
   #1 == 2 b  c

            2  2
   #2 == 2 a  c

            2  2
   #3 == 2 a  b


                3       3       3           4      4        4    4        4    4      5    5    5      2  3      3  2      2  3      3  2        2  2      2    2      2
-((a - b + c) (a  #1 - b  #1 + c  #1 - 3 a b  + 3 a  b + a c  - a  c + b c  + b  c + a  - b  - c  - 2 a  b  + 2 a  b  + 2 a  c  - 2 a  c  - 2 a b  c  - 4 a  b c  - a b  #1

      2           2       2           2       2               3        3        3           2
   + a  b #1 + a c  #1 + a  c #1 - b c  #1 + b  c #1 + 2 a b c  + 2 a b  c - 2 a  b c))/(4 a  (a + b + c) #1)

where

   #1 == sqrt((a + b + c) (a + b - c) (a - b + c) (b - a + c))


>> solved
 3    2      2        2      2    3    2        2    3
a  + a  b + a  c - a b  + a c  - b  + b  c - b c  + c
------------------------------------------------------
                    2 a (a + b + c)

   4      2  2      2          2  2    4      3        2  2        3    4
  a  - 2 a  b  + 2 a  b c - 2 a  c  + b  - 2 b  c + 2 b  c  - 2 b c  + c
- -----------------------------------------------------------------------
         2 a sqrt((a + b + c) (a + b - c) (a - b + c) (b - a + c))


ans =

[-1, a^3 + a^2*b + a^2*c - a*b^2 + a*c^2 - b^3 + b^2*c - b*c^2 + c^3]


ans =

[a - b + c, a + b - c, a^2 - b^2 - c^2]

 3    2      2        2      2    3    2        2    3
a  + a  b + a  c - a b  + a c  - b  + b  c - b c  + c
------------------------------------------------------
                    8 a (a + b + c)

   4           2             4      3               3    4
  a  - #3 + 2 a  b c - #2 + b  - 2 b  c + #1 - 2 b c  + c
- --------------------------------------------------------
                       4              4         4
           8 a sqrt(- a  + #3 + #2 - b  + #1 - c )

where

            2  2
   #1 == 2 b  c

            2  2
   #2 == 2 a  c

            2  2
   #3 == 2 a  b


0

>>
```

---

### 01/21/2022

#### There are five stones $A, B, C, D, E$ in a pond. A frog can jump from one stone to any other stone except current one. It starts from stone $A$. What is the possibility that it is back on stone $A$ after $5$ jumps?

**Solve 1:**

The transfer matrix is:
$$
\begin{align*}
A=
\begin{vmatrix}
0 & \dfrac{1}{4} & \dfrac{1}{4} & \dfrac{1}{4} & \dfrac{1}{4} \\
\dfrac{1}{4} & 0 & \dfrac{1}{4} & \dfrac{1}{4} & \dfrac{1}{4} \\
\dfrac{1}{4} & \dfrac{1}{4} & 0 & \dfrac{1}{4} & \dfrac{1}{4} \\
\dfrac{1}{4} & \dfrac{1}{4} & \dfrac{1}{4} & 0 & \dfrac{1}{4} \\
\dfrac{1}{4} & \dfrac{1}{4} & \dfrac{1}{4} & \dfrac{1}{4} & 0
\end{vmatrix} \\ .

A^5 =
\begin{vmatrix}
\dfrac{51}{256} & \dfrac{205}{1024} & \dfrac{205}{1024} & \dfrac{205}{1024} & \dfrac{205}{1024} \\
\dfrac{205}{1024} & \dfrac{51}{256} & \dfrac{205}{1024} & \dfrac{205}{1024} & \dfrac{205}{1024} \\
\dfrac{205}{1024} & \dfrac{205}{1024} & \dfrac{51}{256} & \dfrac{205}{1024} & \dfrac{205}{1024} \\
\dfrac{205}{1024} & \dfrac{205}{1024} & \dfrac{205}{1024} & \dfrac{51}{256} & \dfrac{205}{1024} \\
\dfrac{205}{1024} & \dfrac{205}{1024} & \dfrac{205}{1024} & \dfrac{205}{1024} & \dfrac{51}{256}
\end{vmatrix}
\end{align*}
$$.

So the possibility that the frog is back to stone $A$ is $\boxed{\dfrac{51}{256}}$.

**Solve 2:**

Jump 1，there are $4^1$ situations，$\dfrac{0}{4}$ on $A$.  So $4^1-0=4$ on non-$A$.
Jump 2,  $\dfrac{4}{4^2}$ on $A$. So $4^2-4=12$ on non-$A$.
Jump 3,  $\dfrac{12}{4^3}$ on $A$. So $4^3-12=52$ on non-$A$.
Jump 4,  $\dfrac{52}{4^4}$ on $A$. So $4^4-52=204$ on non-$A$.
Jump 5,  $\dfrac{204}{4^5}=\dfrac{51}{256}$ on $A$.

So the possibility that the frog is back to stone $A$ is $\boxed{\dfrac{51}{256}}$.

---
