---
title: Oct 2022
date: 2022-10-06 01:00
tags: []
---

#### 10/06/2022

#### What are the last three digits of $7^{2022}$?

**Solve:**
$$
\begin{multline}\nonumber
\shoveleft \text{The last three digits of }7^{2022} \text{ is the same as } (7^{2022}\mod{1000})\\
\shoveleft \text{By Euler's totient function we know:}\\
\shoveleft \implies \varphi(1000)=\varphi(2^3\cdot 5^3)=(2^3-2^2)\cdot(5^3-5^2)=400\\
\shoveleft \implies 7^{\varphi(1000)} \equiv 1 \mod{1000}\\
\shoveleft \implies 7^{400} \equiv 1 \mod{1000}\\
\shoveleft \implies 7^{2022}=7^{2000} \cdot 7^{22}=7^{2022}\cdot(50-1)^{11}\\
\shoveleft \implies 7^{2022} \mod{1000}=(50-1)^{11} \mod{1000}\\
\shoveleft \implies 7^{2022} \mod{1000}\equiv {11 \choose 9} 50^2(-1)^9+{11 \choose 10} 50(-1)^{10}+{11 \choose 11}(-1)^{11} \mod{1000}\\
\shoveleft \implies 7^{2022} \mod{1000}\equiv -500+11\cdot50-1\equiv49\mod{1000}\\
\shoveleft \implies \text{the last three digits of }7^{2022} \text{ are } \bbox[5px, border: 1px solid black]{049}.
\end{multline}
$$
**Note:**

* [Fermat's little Theorem](https://en.wikipedia.org/wiki/Fermat%27s_little_theorem): $p$ is prime $\implies a^p \equiv a \mod{p}$.
* If $p$ is prime, $gcd(a,p)=1 \implies a^{p-1}\equiv 1 \mod{p}$.
* With [Euler's totient function](https://en.wikipedia.org/wiki/Euler%27s_totient_function), $p$ is prime $\implies \varphi(p)=p-1$. If $gcd(a,p)=1 \implies a^{\varphi(n)} \equiv 1 \mod{n}$
* $n=p_{1}^{k_1}\cdotp_{2}^{k_2}\cdot \dots\cdot p_{m}^{k_m} \implies \varphi(n)=(p_{1}^{k_1}-p_{1}^{k_1-1})(p_{2}^{k_2}-p_{2}^{k_2-1})\dots (p_{n}^{k_n}-p_{n}^{k_n-1}) \text{ where }p_i \text{ is prime for }i=1,2 \dots m$

---

#### 10/11/2022

#### Simplify $\cfrac{1+\sqrt{2-\sqrt{2}}+\sqrt{2-\sqrt{3}}}{\sqrt{3}+\sqrt{2+\sqrt{2}}+\sqrt{2+\sqrt{3}}}$

**Solve:**
$$
\begin{multline}\nonumber
\shoveleft \text{Notice that} \cfrac{1+\sqrt{2-\sqrt{2}}+\sqrt{2-\sqrt{3}}}{\sqrt{3}+\sqrt{2+\sqrt{2}}+\sqrt{2+\sqrt{3}}}=\cfrac{\sqrt{2-\sqrt{1}}+\sqrt{2-\sqrt{2}}+\sqrt{2-\sqrt{3}}}{\sqrt{2+\sqrt{1}}+\sqrt{2+\sqrt{2}}+\sqrt{2+\sqrt{3}}}\\
\shoveleft \text{Generally consider }\cfrac{\displaystyle\sum_{k=1}^{n^2-1}{\sqrt{n-\sqrt{k}}}}{\displaystyle\sum_{k=1}^{n^2-1}{\sqrt{n+\sqrt{k}}}}, n,k \in \mathbb{N^*}, \text{we can prove that}\\
\shoveleft \sqrt{n-\sqrt{k}}+\sqrt{n+\sqrt{k}}=\sqrt{n-2\sqrt{\cfrac{k}{4}}}+\sqrt{n+2\sqrt{\cfrac{k}{4}}}=\sqrt{2}\sqrt{n+\sqrt{n^2-k}}\\
\shoveleft \text{Consider }n \text{ as roots of quadratic equation } X^2-nX+\cfrac{k}{4}=0\\
\shoveleft \text{where } X_1+X_2=n, X_1X_2=\cfrac{k}{4} \implies X=\cfrac{n\pm\sqrt{n^2-k}}{2} \\
\shoveleft \implies n-2\sqrt{\cfrac{k}{4}}=\Biggl( \sqrt{\cfrac{n+\sqrt{n^2-k}}{2}}-\sqrt{\cfrac{n-\sqrt{n^2-k}}{2}} \Biggr)^2\\
\shoveleft \implies n+2\sqrt{\cfrac{k}{4}}=\Biggl( \sqrt{\cfrac{n+\sqrt{n^2-k}}{2}}+\sqrt{\cfrac{n-\sqrt{n^2-k}}{2}} \Biggr)^2\\
\shoveleft \implies\sqrt{n-\sqrt{k}}+\sqrt{n+\sqrt{k}}=2\sqrt{\cfrac{n+\sqrt{n^2-k}}{2}}=\sqrt{2}\sqrt{n+\sqrt{n^2-k}}\\
\shoveleft \text{Now we check: } \cfrac{\displaystyle\sum_{k=1}^{n^2-1}{\sqrt{n-\sqrt{k}}}}{\displaystyle\sum_{k=1}^{n^2-1}{\sqrt{n+\sqrt{k}}}} = \cfrac{\displaystyle\sum_{k=1}^{n^2-1}{\Bigl(\sqrt{n-\sqrt{k}}}+\sqrt{n+\sqrt{k}}\Bigr)}{\displaystyle\sum_{k=1}^{n^2-1}{\sqrt{n+\sqrt{k}}}}-1\\
\shoveleft = \cfrac{\displaystyle\sum_{k=1}^{n^2-1}{\sqrt{2}\sqrt{n+\sqrt{n^2-k}}}}{\displaystyle\sum_{k=1}^{n^2-1}{\sqrt{n+\sqrt{k}}}}-1 \xlongequal[]{i=n^2-k} \sqrt{2}\cdot \cfrac{\displaystyle\sum_{i=n^2-1}^{1}{\sqrt{n+\sqrt{i}}}}{\displaystyle\sum_{k=1}^{n^2-1}{\sqrt{n+\sqrt{k}}}}-1=\sqrt{2}-1\\
\shoveleft \text{So as special case, }n=2: \cfrac{1+\sqrt{2-\sqrt{2}}+\sqrt{2-\sqrt{3}}}{\sqrt{3}+\sqrt{2+\sqrt{2}}+\sqrt{2+\sqrt{3}}}=\bbox[5px, border: 1px solid black]{\sqrt{2}-1}\\
\end{multline}
$$

---

