---
title:
date: 2022-04-04 12:47
tags: []

---

### 2022-04-04

#### In $\triangle{ABC}$, $\angle{ABC}=48^{\circ}, \angle{ACB}=30^{\circ}$. Extend $BC$ t0 $D$ so that $AB=CD$. Find $\angle{ADC}$.

![image-20220404125034395](/assets/images/2022-04/image-20220404125034395.png)

**Solve:**

![image-20220404130506938](/assets/images/2022-04/image-20220404125258142.png)

Make $F$ on $BC$ so that $\angle{AFB}=\angle{ABF}=48^{\circ}$. Make equilateral triangle $\triangle{AGF}$. Connect $BG, CG, DG$.

Easy to see $AB=AF=AG=FG$, $\angle{AGF}=60^{\circ}=2 \cdot \angle{ACF}, AG=FG \implies $

$G$ is the circumcenter of $\triangle{ACF} \implies CG=FG=AG=AF=AB$

$\angle{GFC}=180^{\circ}-48^{\circ}-60^{\circ}=72^{\circ} \implies \angle{FGC}=36^{\circ}, \angle{FCG}=72^{\circ} \implies \angle{CDG}=\angle{CGD}=36^{\circ} $

$\implies \angle{FGD}=72^{\circ}=\angle{GFD} \implies \triangle{ADG} \cong \triangle{ADF} \implies \angle{ADC}=\dfrac{\angle{FDG}}{2}=\boxed{18^{\circ}}$

---

### 2022-04-10

#### Solve the equation group in real numbers:
$$
\begin{equation}
\begin{cases}
x^3+2x-y=1 \\
y^3+y+x=11
\end{cases}
\end{equation}
$$

**Solve:**

$x^2+2x-y=1 \implies x^3+2x-3=y-2 \implies (x-1)(x^2+x+3)=y-2$
$x \in \mathbb{R} \implies x^2+x+3 > 0 \implies (x-1)(y-2) \ge 0$
$y^3+y+x=11 \implies y^3+y-10=-(x-1) \implies (y-2)(y^2+2y+5)=-(x-1)$
$y \in \mathbb{R} \implies y^2+2y+5 > 0 \implies (x-1)(y-2) \le 0$
So we know $\boxed{x=1, y=2}$

---

### 2022-04-11

#### $D$ is a point in $\triangle{ABC}$ so that $\angle{ABD}=10^{\circ}, \angle{DBC}=20^{\circ}, \angle{BCD}=40^{\circ}, \angle{DAC}=50^{\circ}$, find $\angle{BAD}$.

![image-20220411175858333](/assets/images/2022-04/image-20220411175858333.png)

**Solve 1:**

This problem is easily done with trigonometric Ceva theorem as:

$\dfrac{sinx}{sin50^{\circ}}\dfrac{sin(60^{\circ}-x)}{sin40^{\circ}}\dfrac{sin20^{\circ}}{sin10^{\circ}}=1 \implies sinx \cdot sin(60^{\circ}-x)=\dfrac{sin50^{\circ}\cdot sin40^{\circ}\cdot sin10^{\circ}}{sin20^{\circ}}$

$=\dfrac{cos40^{\circ} \cdot sin40^{\circ} \cdot sin10^{\circ}}{2sin10^{\circ}\cdot cos10^{\circ}}=\dfrac{sin80^{\circ}}{4cos10^{\circ}}=\dfrac{1}{4} \implies -\dfrac{cos60^{\circ}-cos(2x-60^{\circ})}{2}=\dfrac{1}{4}$

$\implies cos(2x-60^{\circ})=1 \implies 2x-60^{\circ}=0\implies x=\boxed{30^{\circ}}$

**Solve 2:**

![image-20220411182229404](/assets/images/2022-04/image-20220411180410742.png)

Let $E$ be the circumcenter of $\triangle{ACD}$, so $AE=CE=DE, \angle{DEC}=2\angle{DAC}=100^{\circ}$
$\implies \angle{EDC}=\angle{ECD}=40^{\circ}=\angle{BCD} \implies DE \parallel BC$

Extend $ED$ and intersects with $AB$ at $F$, so $\angle{AFE}=\angle{ABC}=30^{\circ}$. Make $G$ on $BC$ so that $\angle{EFG}=100^{\circ}=\angle{FEC} \implies CEFG$ is an isosceles trapezoid $\implies FG=CE$

Let $H$ be the circumcenter of $\triangle{BFG}$, so $BH=GH=FH, \angle{FHG}=2\angle{FBG}=60^{\circ} $
$ \implies \triangle{FGH} \text{ is an equilateral triangle}$
$\implies FH=GH=BH=FG=CE=DE=AE, \angle{HFG}=60^{\circ} $
$ \implies \angle{HBF}=\angle{HFB}=\angle{HFG}-\angle{BFG}=\angle{HFG}-(180^{\circ}-\angle{FBG}-\angle{FGB}) $
$ =\angle{HFG}-(180^{\circ}-\angle{FBG}-\angle{GFE}) =60^{\circ}-(180^{\circ}-100^{\circ}-30^{\circ})=10^{\circ} $
$ \implies FH \parallel BD, \angle{HBD}=20^{\circ}=\angle{DBC}=\angle{FDB} $
$ \implies BDFH \text{ is an isosceles trapezoid} $
$ \implies BH=DF \implies DF=DE=AE$

Check $\triangle{AEF}, \angle{AFE}=30^{\circ}, AE=DE=DF \implies EF=2AE$.

Let $O$ be the circumcenter of $\triangle{AEF}$, so $\angle{AOE}=2 \angle{AFE}=60^{\circ}, AO=FO=EO$

$\implies \triangle{AOE} \text{ is equilateral triangle}$

$ \implies AO=OE=AE=DE=DF=FO=EO $

$ \implies AD=AO=FD $

$ \implies \angle{BAD}=\angle{AFE}=\boxed{30^{\circ}}$

---

### 2022-04-19

#### Point $D$ is in $\triangle{ABC}$ so that $\angle{ABD}=5^{\circ}, \angle{DBC}=20^{\circ}, \angle{DCB}=65^{\circ}, \angle{DAC}=40^{\circ}$, find $\angle{ACD}$.

![image-20220419155421788](/assets/images/2022-04/image-20220419155302818.png)

**Solve 1:**

Trigonometric Ceva theorem approach is quite straight forward:

$$
\begin{multline}
\shoveleft \dfrac{sin(50^{\circ}-x)}{sin40^{\circ}}\dfrac{sinx}{sin65^{\circ}}\dfrac{sin20^{\circ}}{sin5^{\circ}}=1 \\
\shoveleft \implies sin(50^{\circ}-x)sinx=\dfrac{sin5^{\circ} \cdot sin40^{\circ}\cdot sin65^{\circ}}{sin20^{\circ}}=2sin5^{\circ}\cdot cos20^{\circ} \cdot sin65^{\circ}\\
\shoveleft \implies cos(50^{\circ}-2x)-cos50^{\circ}=4sin5^{\circ} \cdot cos20^{\circ} \cdot cos 25^{\circ} \\
\shoveleft \implies cos(50^{\circ}-2x)=4sin5^{\circ} \cdot cos20^{\circ} \cdot cos 25^{\circ}+sin40^{\circ}\\
 \shoveleft \qquad =4sin5^{\circ} \cdot cos20^{\circ} \cdot cos 25^{\circ}+2sin20^{\circ}\cdot cos20^{\circ}\\
 \shoveleft \qquad =2cos20^{\circ}(2sin5^{\circ}sin65^{\circ}+cos70^{\circ})\\
 \shoveleft \qquad =2cos20^{\circ}(cos60^{\circ}-cos70^{\circ}+cos70^{\circ})\\
 \shoveleft \qquad =cos20^{\circ}\\
\shoveleft \implies 50^{\circ}-2x=\pm 20^{\circ} \\
\shoveleft \implies x=\boxed{15^{\circ}} \text{ or } x=\boxed{35^{\circ}} \nonumber
\end{multline}
$$
**Solve 2:**

---





