---
title: November 2023
date: 2023-11-01 01:47
tags: []
---

### 11/01/2023

#### Morley's Theorem: the three points of intersection of the adjacent angle trisectors of any triangle form an equilateral triangle.

![image-20231101020158661](/assets/images/2023/image-20231101020158661.png)

**Prove:**

![image-20231108215829814](/assets/images/2023/image-20231108215829814.png)

![image-20231108221245268](/assets/images/2023/image-20231108221245268.png)
$$
\begin{multline}\nonumber
\shoveleft \text{This approval is originated from John conway.}\\
\shoveleft \text{Suppose for any angles }\alpha, \beta, \gamma \text{ such that }\alpha+\beta+\gamma=60^{\circ}\\
\shoveleft \text{ seven triangles can be constructed as above where}\\
\shoveleft 0^{+}=60^{\circ}, \alpha^{+}=\alpha+60^{\circ}, \alpha^{++}=\alpha+120^{\circ}, \text{ etc} \implies \\
\shoveleft\triangle{A_1P_2R_1'}\cong\triangle{A_2P_3R_1}\cong\triangle{A_3R_2P_3'}\\
\shoveleft \triangle{B_1P2Q_3'}\cong\triangle{B_2P_1Q_3}\cong\triangle{B_3Q_2P_1'}\\
\shoveleft \triangle{C_1R_2Q_1'}\cong\triangle{C_2R_3Q_1}\cong\triangle{C_3R_3'Q_2}\\
\shoveleft \implies P_2R_1'=P_3R_1=R_2P_3'=PR=P_2Q_3'=P_1Q_3=P_1'Q_2=PQ=R_3'Q_2=R_3Q_1=R_2Q_1'=QR\\
\shoveleft \implies \triangle{PQR} \text{ is equilateral}\implies \text{The construction is unique and determined}\\
\shoveleft \implies \text{The seven triangles can be combined to a triangle}\\
\shoveleft \implies \text{This means for any triangle, its adjacent angle trisectors form an equilateral triangle.}\blacksquare
\end{multline}
$$

---

### 11/02/2023

#### Point $E, F$ are on side $AB, AD$ of rectangle $ABCD$ such that $EF=CF, \angle{EFC}=120^{\circ}, [AEF]=M, [BCE]=N$, find $[CDF]$

![image-20231102072634776](/assets/images/2023/image-20231102072441652.png)

**Solve:**

![image-20231102072752847](/assets/images/2023/image-20231102072752847.png)
$$
\begin{multline}\nonumber
\shoveleft \text{Let }EF=CF=b, \angle{DCF}=\alpha \implies CE=\sqrt{3}b \\
\shoveleft \angle{AFE}=\alpha-30^{\circ}, \angle{BCE}=60^{\circ}-\alpha \implies\\
\shoveleft [AEF]=\dfrac{b^2\cdot sin(\alpha-30^{\circ})\cdot cos(\alpha-30^{\circ})}{2}\\
\shoveleft =\dfrac{b^2sin(2\alpha-60^{\circ})}{4}=M \implies sin(2\alpha-60^{\circ})=\dfrac{4M}{b^2}\\
\shoveleft \implies sin(2\alpha)cos60^{\circ}-cos(2\alpha)sin60^{\circ}=\dfrac{4M}{b^2}\\
\shoveleft [BCE]=\dfrac{3b^2\cdot sin(60^{\circ}-\alpha)\cdot cos(60^{\circ}-\alpha)}{2}\\
\shoveleft =\dfrac{3b^2sin(120^{\circ}-2\alpha)}{4}=N\implies sin(120^{\circ}-2\alpha)=\dfrac{4N}{3b^2}\\
\shoveleft \implies sin(2\alpha+60^{\circ})=\dfrac{4N}{3b^2}\implies sin(2\alpha)cos60^{\circ}+cos(2\alpha)sin60^{\circ}=\dfrac{4N}{3b^2}\\
\shoveleft [CDF]=\dfrac{b^2\cdot sin(\alpha)\cdot cos(\alpha)}{2}=\dfrac{b^2sin(2\alpha)}{4}=\dfrac{b^2(\dfrac{4M}{b^2}+\dfrac{4N}{3b^2})}{4}=\bbox[5px, border: 1px solid black]{M+\dfrac{N}{3}}
\end{multline}
$$

---

### 11/04/2023

#### $E,F$ are points on side $AD, AB$ of square $ABCD$ such that $\angle{AEF}=\angle{CEF}$,$[CBF]=4$, $[CEF]=5$, find $[CDE]$.

![image-20231104061857887](/assets/images/2023/image-20231104061857887.png)

**Solve:**

![image-20231105023141644](/assets/images/2023/image-20231105023141644.png)
$$
\begin{multline}\nonumber
\shoveleft \text{Let }AF=a, BF=b, \angle{AEF}=\angle{CEF}=\alpha, \text{Extend }EF, CB \text{ and intersect at }G\\
\shoveleft \implies CD=BC=a+b, AE=\dfrac{a}{tan \alpha}, BG=\dfrac{b}{tan \alpha}, DE=a+b-\dfrac{a}{tan\alpha}\\
\shoveleft [BCF]=\dfrac{b(a+b)}{2}=4\implies \bbox[5px, border: 3px dotted red]{b(a+b)=8} \implies b < 2\sqrt{2}, [CEF]=[CEG]-[CFG]=5\\
\shoveleft \implies \dfrac{(a+b+\dfrac{b}{tan \alpha})a}{2}=5 \implies \bbox[5px, border: 3px dotted red]{tan\alpha=\dfrac{ab^2}{10b-8a}=\dfrac{b^2(8-b^2)}{18b^2-64} \gt 0} \implies 2\sqrt{2} \gt b\gt\dfrac{4a}{5}\\
\shoveleft [CDE]=\dfrac{(a+b)(a+b-\dfrac{a}{tan\alpha})}{2}=\dfrac{(a+b)(4a-b)}{b^2}=\dfrac{\dfrac{256}{b^2}-40}{b^2}\\
\shoveleft \text{For example: } a=b=2, tan\alpha=2, [CDE]=6; \text{If claim } a=b, \text{ then this is the only solution.}\\
\shoveleft \text{Otherwise, for example: }b=2.05, a=\dfrac{8}{2.05}-2.05=1.852439, b^2=4.2025, tan\alpha=1.37, [CDE]=4.977
\end{multline}
$$

---

### 11/06/2023

#### $D$ is a point on side $BC$ of $\triangle{ABC}$ such that $\angle{DAC}=12^{\circ}, \angle{BAD}= \angle{ACB}=18^{\circ}$, show that $AB=CD$.

![image-20231106130003362](/assets/images/2023/image-20231106130003362.png)

**Prove:**

![image-20231106124415980](/assets/images/2023/image-20231106124415980.png)
$$
\begin{multline}\nonumber
\shoveleft \text{Let }E \text{ be the circum-center of }\triangle{ABD}, BE \text{ and } AC \text{ intersect at } F\\
\shoveleft \angle{BAD}=18^{\circ},\angle{ADB}=30^{\circ} \implies \angle{BED}=36^{\circ}, \triangle{AEB} \text{ is equilateral}\\
\shoveleft \implies AB=AE=BE=DE, \angle{EBD}=\angle{EDB}=\dfrac{180^{\circ}-36^{\circ}}{2}=72^{\circ}\\
\shoveleft \angle{BAF}=30^{\circ}\implies AC\perp BE, BF=EF \implies \triangle{CEF}\cong\triangle{CBF}\\
\shoveleft \implies \angle{CEF}=\angle{CBF}=72{^\circ} \implies \angle{CED}=\angle{ECD}=36^{\circ}\implies CD=DE=AB\blacksquare
\end{multline}
$$

---

### 11/07/2023

#### $D$ is the mid point of side $BC$ of $\triangle{ABC}$, and $\angle{B}=30^{\circ}, \angle{C}=15^{\circ}$. Find $\angle{CAD}$.

![image-20231107012247835](/assets/images/2023/image-20231107012247835.png)

**Solve:**

![image-20231107012210732](/assets/images/2023/image-20231107012210732.png)
$$
\begin{multline}\nonumber
\shoveleft \text{Let } E \text{ the circum-center of }\triangle{ABC} \implies \\
\shoveleft AE=BE=CE, \angle{AEB}=30^{\circ}, \angle{AEC}=60^{\circ}\\
\shoveleft \implies \triangle{ACE}\text{ is equilateral}\implies AE=AC\\
\shoveleft \angle{ABE}=\angle{BAE}=75^{\circ}\implies \angle{CBE}=\angle{BCE}=45^{\circ}\\
\shoveleft \implies BD=DE=CD \implies \triangle{ADE}\cong\triangle{ADC}\\
\shoveleft \implies \angle{CAD}=\angle{EAD}=\dfrac{60^{\circ}}{2}=\bbox[5px, border: 1px solid black]{30^{\circ}}
\end{multline}
$$

---

### 11/08/2023

#### $\triangle{ABC}$ has $AB=6, BC=10, \angle{B}=90^{\circ}$. $D$ is midpoint of side $AB$, and $E$ is a point on $BC$ such that AE and CD intersect at $F$, $\angle{CFE}=45^{\circ}$, find $BE$.

![image-20231108004311680](/assets/images/2023/image-20231108004311680.png)

**Solve 1:**

![image-20231108004205525](/assets/images/2023/image-20231108002233539.png)
$$
\begin{multline}\nonumber
\shoveleft \text{Make }AP\perp CD \text{ at }P, EQ \perp CD \text{ at }Q\\
\shoveleft \triangle{ADP}\sim\triangle{CDB}\implies AP=\dfrac{24}{\sqrt{73}}, DP=\dfrac{9}{\sqrt{73}}\\
\shoveleft \implies DF=PF-PD=AP-PD=\dfrac{15}{\sqrt{73}}\\
\shoveleft \text{Let }FQ=EQ=b, CD=\sqrt{73},CQ=\sqrt{73}-\dfrac{15}{\sqrt{73}}-b\\
\shoveleft \triangle{CEQ}\sim \triangle{CDB}\implies \dfrac{\sqrt{73}-\dfrac{15}{\sqrt{73}}-b}{b}=\dfrac{8}{3}\\
\shoveleft \implies b=\dfrac{174}{11\sqrt{73}}\implies \dfrac{CE}{\dfrac{174}{11\sqrt{173}}}=\dfrac{\sqrt{73}}{3}\\
\shoveleft \implies CE=\dfrac{58}{11}\implies BE=\bbox[5px, border: 1px solid black]{\dfrac{30}{11}}
\end{multline}
$$
**Solve 2:**
$$
\begin{multline}\nonumber
\shoveleft tan(\angle{AEB})=tan(45^{\circ}+\angle{BCD})\\
\shoveleft =\dfrac{tan45^{\circ}+tan(\angle{BCD})}{1-tan45^{\circ}\cdot tan(\angle{BCD})}\\
\shoveleft =\dfrac{1+\dfrac{3}{8}}{1-\dfrac{3}{8}}=\dfrac{11}{5}=\dfrac{AB}{BE}=\dfrac{6}{BE}\\
\shoveleft \implies BE=\bbox[5px, border: 1px solid black]{\dfrac{30}{11}}
\end{multline}
$$

---

### 11/09/2023

#### In quadrilateral $ABCD$, $\angle{ABC}=38^{\circ}, \angle{CBD}=44^{\circ}, \angle{CAD}=22^{\circ},\angle{BAD}=16^{\circ}$, find $\angle{ADC}$.

![image-20231108015106962](/assets/images/2023/image-20231108015106962.png)

**Solve:**

![image-20231108021306099](/assets/images/2023/image-20231108020300491.png)
$$
\begin{multline}\nonumber
\shoveleft \text{It can be generalized to above figure. Easy to see }AB=AD, AC=BC.\\
\shoveleft AB=AD \implies \text{Make }C' \text{ below } AB \text{ such that }\triangle{AC'B}\cong\triangle{ACD} \implies\\
\shoveleft \angle{C'AB}=\angle{CAD}=\alpha, AC=AC'\implies \triangle{ACC'}\text{ is equilateral}\\
\shoveleft \implies CC'=AC=AC'=BC \implies C \text{ is the circum-center of }\triangle{ABC'}\\
\shoveleft \implies \angle{BCC'}=2\angle{C'AB}=2\alpha\implies \angle{CBC'}=\dfrac{180^{\circ}-2\alpha}{2}=90^{\circ}-\alpha\\
\shoveleft \implies \angle{ABC'}=90^{\circ}-\alpha-(60^{\circ}-\alpha)=30^{\circ}\implies \angle{ADC}=\bbox[5px, border: 1px solid black]{30^{\circ}}
\end{multline}
$$

---

### 11/10/2023

#### $E,F$ are on side $AB, BC$ of square $ABCD$ respectively such that $\angle{EDF}=45^{\circ}$. $DE, DF$ intersect with $AC$ at $H,G$ respectively such that $AH=20, CG=21$. Find $GH$.

![image-20231108192953069](/assets/images/2023/image-20231108192953069.png)

**Solve:**

![image-20231108203050122](/assets/images/2023/image-20231108203050122.png)
$$
\begin{multline}\nonumber
\shoveleft \text{Rotate }\triangle{ADE} \text{ clockwise for } 90^{\circ}\text{ to get }\triangle{CDE'} \text{ where } H \text{ is mapped to }H'.\\
\shoveleft \implies AH=CH'=20,DH=DH', \angle{GDH'}=45^{\circ}=\angle{GDH}\\
\shoveleft \implies \triangle{DGH}\cong\triangle{DGH'}\implies GH=GH'\\
\shoveleft \text{Easy to see that }\angle{GCH'}=90^{\circ}\implies GH=GH'=\sqrt{20^2+21^2}=\bbox[5px, border: 1px solid black]{29}\\
\shoveleft
\end{multline}
$$

---

### 11/11/2023

#### $D,E$ are points in side $BC, CA$ respectively of $\triangle{ABC}$ such that $BD=8$, $DE=7, $$AD=CD$, $\angle{CDE}=2\angle{BAD}, $$\angle{ADE}=60^{\circ}$, find $AE$

![image-20231110223136875](/assets/images/2023/image-20231110223136875.png)

**Solve 1:**

![image-20231110223040915](/assets/images/2023/image-20231110223040915.png)
$$
\begin{multline}\nonumber
\shoveleft \text{Let }AE=x, AD=CD=m, CE=n, \angle{BAD}=\alpha \implies\\
\shoveleft \angle{CDE}=2\alpha, \angle{ADB}=180^{\circ}-60^{\circ}-2\alpha=2\angle{CAD}=2\angle{ACD}\\
\shoveleft \implies \angle{CAD}=\angle{ACD}=60^{\circ}-\alpha \implies \angle{BAC}=60^{\circ}, \angle{AED}=60^{\circ}+\alpha\\
\shoveleft \implies \dfrac{7}{sin(60^{\circ}-\alpha)}=\dfrac{x}{sin60^{\circ}}=\dfrac{m}{sin(60^{\circ}+\alpha)}\\
\shoveleft \dfrac{8}{sin\alpha}=\dfrac{m}{sin(120^{\circ}-2\alpha+\alpha)}=\dfrac{m}{sin(60^{\circ}+\alpha)}\\
\shoveleft \implies \dfrac{x}{sin60^{\circ}}=\dfrac{8}{sin\alpha}=\dfrac{7}{sin60^{\circ}cos\alpha-cos60^{\circ}sin\alpha}\implies tan\alpha=\dfrac{4\sqrt{3}}{11}\\
\shoveleft \implies cos\alpha=\dfrac{11}{13}, cos\alpha=\dfrac{4\sqrt{3}}{13}\implies sin(60^{\circ}-\alpha)=\dfrac{7\sqrt{3}}{26}\\
\shoveleft \implies x=\dfrac{\dfrac{7\sqrt{3}}{2}}{\dfrac{7\sqrt{3}}{26}}=\bbox[5px, border: 1px solid black]{13}
\end{multline}
$$
**Solve 2:**

![image-20231110230146111](/assets/images/2023/image-20231110230146111.png)
$$
\begin{multline}\nonumber
\shoveleft \text{Let }\angle{BAD}=\alpha \implies \angle{CDE}=2\alpha, \angle{ADB}=180^{\circ}-60^{\circ}-2\alpha=2\angle{CAD}=2\angle{ACD}\\
\shoveleft \implies \angle{CAD}=\angle{ACD}=60^{\circ}-\alpha \implies \angle{BAC}=60^{\circ}, \angle{AED}=60^{\circ}+\alpha\\
\shoveleft \text{Notice that a triangle with side length 7,8,13 has an angle } 120^{\circ}, cos120^{\circ}=\dfrac{49+64-169}{2\times7\times 8}\\
\shoveleft \text{Extend } AD \text{ to } F \text{ such that } BD=FD=8, \angle{EDF}=120^{\circ}\implies EF=13\\
\shoveleft \triangle{ABD}\cong\triangle{CFD}\implies \angle{BAD}=\angle{FCD}=\alpha\implies \angle{ECF}=60^{\circ}=\angle{ADE}\\
\shoveleft \implies CEDF \text{ is cyclic}\implies \angle{EFD}=\angle{ECD}=\angle{CAD}\implies AE=EF=\bbox[5px, border: 1px solid black]{13}
\end{multline}
$$

**Note:**

- A triangle with sides $7, 8, 13$ has angle $120^{\circ}$

---

### 11/12/2023

#### $D,E,F$ are points on side $AB,BC,CA$ respectively of right angle triangle $\triangle{ABC}$ , where $DE\parallel AC, BD=18, CF=10$, find $[BEF]$

![image-20231111141941543](/assets/images/2023/image-20231111141941543.png)

**Solve:**
$$
\begin{multline}\nonumber
\shoveleft [BEF]=[BCF]-[CEF]=\dfrac{CF \cdot AB}{2}-\dfrac{CF\cdot AD}{2}=\dfrac{CF \cdot BD}{2}=\dfrac{18\cdot10}{2}=\bbox[5px, border: 1px solid black]{90}
\end{multline}
$$

---

### 11/13/2023

#### $P,Q$ are two points outside of circle $\odot O$. $A,B,C$ are points on the circle $\odot O$. $PQ, PA, QB$ are tangent to the circle. $AC=BC$. $CP, CQ$intersect with $AB$ at $D,E$. Show that $AB=2DE$.

![image-20231112105312922](/assets/images/2023/image-20231112105312922.png)

**Prove 1:**

![image-20231114222205538](/assets/images/2023/image-20231114222205538.png)
$$
\begin{multline}\nonumber
\shoveleft \triangle{PFM}\sim\triangle{PCF}\implies \dfrac{FM}{FC}=\dfrac{PF}{PC}=\dfrac{PA}{PC}\implies \dfrac{AM}{AC}=\dfrac{FM}{FC}\\
\shoveleft \triangle{AMC}\sim\triangle{DAC}\implies AC^2=CD\cdot CM, \dfrac{DA}{DC}=\dfrac{AM}{AC} \implies \dfrac{DA}{DC}=\dfrac{FM}{FC}\\
\shoveleft \triangle{AFC}\sim\triangle{GAC}\implies AC^2=FC \cdot CG \implies \dfrac{CD}{CG}=\dfrac{FC}{CM}\\
\shoveleft \implies \triangle{CDG}\sim\triangle{CFM}\implies \dfrac{DG}{DC}=\dfrac{FM}{FC}=\dfrac{DA}{DC}\implies DG=DA\\
\shoveleft \text{Similarly } BE=GE\implies AB=AD+DG+BE+GE=2DE\blacksquare
\end{multline}
$$

**Prove 2 (better expressed):**
$$
\begin{multline}\nonumber
\shoveleft \triangle{PAM}\sim\triangle{PCA},\triangle{PFM}\sim\triangle{PCF}\implies \dfrac{AM}{AC}=\dfrac{PA}{PC}=\dfrac{PF}{PC}=\dfrac{FM}{FC}\\
\shoveleft \triangle{AMC}\sim\triangle{DAC}\implies \dfrac{DA}{DC}=\dfrac{AM}{AC}=\dfrac{FM}{FC}\\
\shoveleft \angle{CDG}=\angle{DAC}+\angle{ACD}=\angle{AFG}+\angle{MFA}=\angle{MFG}\\
\shoveleft \implies \triangle{CDG}\sim\triangle{CFM} \implies \dfrac{DG}{DC}=\dfrac{FM}{FC}=\dfrac{DA}{DC}\implies DA=DG\\
\shoveleft \text{Similarly } BE=GE\implies AB=AD+DG+BE+GE=2DE\blacksquare
\end{multline}
$$

---



### 11/14/2023

#### Two circles intersect at $A,D$, $B,C$ are points on one circle and $P,Q$ are points on the other. $B,P,Q,C$ are colinear. Prove that $\angle{BAP}=\angle{CDQ}$.

![image-20231114125013991](/assets/images/2023/image-20231114125013991.png)

**Prove 1:**

![image-20231114124328392](/assets/images/2023/image-20231114124328392.png)
$$
\begin{multline}\nonumber
\shoveleft \text{Extend }AP, DQ \text{ and intersect with the circle at }E, F. \text{ Connect }CE.\\
\shoveleft APQD \text{ is cyclic }\implies \angle{PAD}=\angle{PQF}\\
\shoveleft AEFD \text{ is cyclic }\implies \angle{PAD}+\angle{EFQ}=180^{\circ}\\
\shoveleft \implies \angle{PQF}+\angle{EFQ}=180^{\circ}\implies BC\parallel EF\\
\shoveleft \implies \angle{BAP}=\angle{BCE}=\angle{CEF}=\angle{CDQ}\blacksquare
\end{multline}
$$
**Prove 2:**
$$
\begin{multline}\nonumber
\shoveleft \angle{APQ}+\angle{ADQ}=180^{\circ}=\angle{ABP}+\angle{ADC}\\
\shoveleft \implies \angle{APQ}-\angle{ABP}=\angle{ADC}-\angle{ADQ}\\
\shoveleft \implies \angle{BAP}=\angle{CDQ}\blacksquare
\end{multline}
$$

---

### 11/15/2023

#### $D,F,G$ are points on side $AC,AB,BC$ of $\triangle{ABC}$ respectively. extended $DF, CB$ intersect at $E$, extended $DG,AB$ intersect at $F$, $[AEF]=M$, $[BEF]=N$, $[BFG]=P$,$[CFG]=Q$, find $X=[ADF]$,$Y=[BFDG]$,$Z=[CDG]$

![image-20231114140726225](/assets/images/2023/image-20231114140407828.png)

**solve:**

![image-20231115162101075](/assets/images/2023/image-20231115162101075.png)
$$
\begin{multline}\nonumber
\shoveleft \dfrac{P+Q}{S}=\dfrac{(M+N)x+(P+Q)y}{M+N}\implies S=\dfrac{(P+Q)(M+N)}{(M+N)x+(P+Q)y}\\
\shoveleft \dfrac{Mx}{M}=x=\dfrac{P+Nx+Py}{S+N}\implies Sx=(1+y)P \implies S=\dfrac{(1+y)P}{x}\\
\shoveleft \dfrac{Qy}{Q}=y=\dfrac{N+Nx+Py}{S+P}\implies Sy=(1+x)N \implies S=\dfrac{(1+x)N}{y}\\
\shoveleft \implies \bbox[5px, border: 2px dotted red]{\dfrac{(1+y)P}{x}=\dfrac{(1+x)N}{y}=S}\\
\shoveleft \dfrac{(1+x)M}{(1+x)N+(P+Q)y}=\dfrac{(1+y)P+(M+N)x}{(1+y)Q}=\dfrac{(M+N)x}{(P+Q)y}\\
\shoveleft \implies \dfrac{(1+x)M}{(S+P+Q)y}=\dfrac{(S+M+N)x}{(1+y)Q}=\dfrac{(M+N)x}{(P+Q)y}\implies \\
\shoveleft x=\dfrac{M(P+Q)}{S(M+N)+N(P+Q)}, y=\dfrac{Q(M+N)}{S(P+Q)+P(M+N)}\implies \\
\shoveleft (1+x)N(P+Q)+P(M+N)y=Q(M+N)\\
\shoveleft (1+y)P(M+N)+N(P+Q)x=M(P+Q)\\
\shoveleft \implies \bbox[5px, border: 2px dotted red]{N(P+Q)x+P(M+N)y=MQ-NP}\\
\shoveleft \text{The answer is given by solving equation system: }\\
\shoveleft
\begin{cases}
x(1+x)N=y(1+y)P\\
N(P+Q)x+P(M+N)y=MQ-NP
\end{cases} \\
\shoveleft \text{The result is: }X=Mx, Y=Nx+Py,Z=Qy
\end{multline}
$$
**Solve 2:**
$$
\begin{multline}\nonumber
\shoveleft placeholder
\end{multline}
$$

---

### 11/16/2023

#### Three circles radius as $6,7,8$ are externally tagent to each other. The fourth large circle has the three circles inscribed is tagent to all of them. Find the radius of this larger circle.

![image-20231116133223805](/assets/images/2023/image-20231116133223805.png)

**Solve:**
$$
\begin{multline}\nonumber
\shoveleft \text{Applying Descarte's Theorem: }\\
\shoveleft (\dfrac{1}{r_1}+\dfrac{1}{r_2}+\dfrac{1}{r_3}-\dfrac{1}{r})^2=2(\dfrac{1}{r_1^2}+\dfrac{1}{r_2^2}+\dfrac{1}{r_3^2}+\dfrac{1}{r^2})\\
\shoveleft \text{Let }A=\prod_{cyc}r_i, B=\sum_{cyc}{r_ir_j},C=B^2-2\sum_{cyc}{r_i^2r_j^2}\\
\shoveleft \implies r=\bbox[5px, border: 1px solid black]{\dfrac{A}{C}\Big(B+\sqrt{B^2+C}\Big)}\\
\shoveleft \text{For }r_1=6, r_2=7, r_3=8, A=336, B=146, C=6908\\
\shoveleft \implies r=\dfrac{336}{6908}\Big(146+\sqrt{146^2+6908}\Big)=\bbox[5px, border: 1px solid black]{\dfrac{168}{11}}
\end{multline}
$$

---

### 11/17/2023

#### $D$ is a point inside $\triangle{ABC}$ such that $\angle{BAD}=10^{\circ}$, $\angle{ABD}=\angle{CAD}=20^{\circ}$, $\angle{CBD}=60^{\circ}$, find $\angle{BCD}$.

![image-20231118020431371](/assets/images/2023/image-20231118020431371.png)

**Solve:**

![image-20231118020341011](/assets/images/2023/image-20231118020341011.png)
$$
\begin{multline}\nonumber
\shoveleft \text{Let }F \text{ be the circumcenter of } \triangle{ABC} \implies\\
\shoveleft AF=BF=CF, \angle{BFC}=2\angle{BAC}=60^{\circ}=\angle{DBC}\\
\shoveleft \implies B,D,F \text{ are colinear}, \triangle{BFC}\text{ is equilateral}\\
\shoveleft \implies \angle{FAB}=\angle{FBA}=20^{\circ}\implies \angle{FAD}=\angle{BAD}=10^{\circ}\\
\shoveleft \implies \text{Extend }AF \text{ and intersect } BC \text{ at }G \implies \angle{AGB}=80^{\circ}=\angle{ABG}\\
\shoveleft \implies AB=AG \implies \triangle{BAD}\cong\triangle{GAD}\implies \angle{DGF}=20^{\circ}, BD=BG\\
\shoveleft \implies \triangle{BDG}\text{ is equilateral} \implies DG\parallel CF\implies CGDF \text{ is cyclic}\\
\shoveleft \implies \angle{CDG}=\angle{CFG}=\angle{DGF}=20^{\circ}\\
\shoveleft \implies \angle{BCD}=180^{\circ}-60^{\circ}-60^{\circ}-20^{\circ}=\bbox[5px, border: 1px solid black]{40^{\circ}}
\end{multline}
$$

---

### 11/18/2023

#### $\displaystyle\sum_{n=1}^{\infty}{\dfrac{1}{n^4}}=?$

**Solve 1:**
$$
\begin{multline}\nonumber
\shoveleft \text{Recall that the Fourier series for a } 2\pi \text{-periodic function }f \text{ has the complex form}\\
\shoveleft S(x)=\displaystyle \sum_{n=-\infty}^{\infty}{c_ne{inx}}, \quad c_n=(f, e_n)=\dfrac{1}{2\pi}\int_{-\pi}^{\pi}{f(x)e^{-inx}dx}\\
\shoveleft \text{The convergence theorem states that if }f: \mathbb{R} \rightarrow \mathbb{R} \text{ is continuous}, 2\pi \text{-periodic,}\\
\shoveleft \text{and piecewise, then the series converges uniformly on } \mathbb{R}\text{, and }S(x)=f(x) \text{ for all }x \in \mathbb{R}.\\
\shoveleft \text{Taking the limit }N\rightarrow \infty \text{ in the generalized Pythagoream theorem will get}\\
\shoveleft \sum_{n=-\infty}^{\infty}{|c_n|^2}=\dfrac{1}{2\pi}\int_{-\pi}^{\pi}{|f(x)|^2dx}. \text{ This is called Parseval's identity.}\\
\shoveleft \text{To apply this identity, we define }f(x)=x^2 \text{ for } x \in[-\pi, \pi], \text{ then}\\
\shoveleft c_n=(f, e_n)=\dfrac{1}{2\pi}\int_{-\pi}^{\pi}{x^2e^{-inx}dx}=\dfrac{1}{2\pi}\int_{-\pi}^{\pi}{x^2(cos(nx)-isin(nx))dx}=\dfrac{1}{2\pi}\int_{-\pi}^{\pi}{x^2cos(nx)dx}\\
\shoveleft \implies 2\pi c_n=2\int_{0}^{\pi}{x^2cos(nx)dx}=2\Big(x^2\dfrac{sin(nx)}{n}-2x\dfrac{-cos(nx)}{n^2}+2\dfrac{-sin(nx)}{n^3}\Big)\bigg|_{0}^{\pi}=\dfrac{4\pi cos(n\pi)}{n^2}\\
\shoveleft \implies c_n=2\dfrac{(-1)^n}{n^2} \text{for } n \ne 0. \text{ For } n=0 \text{ we have: } c_0=(f, e_0)=\dfrac{1}{2\pi}\int_{-\pi}^{\pi}{x^2dx}=\dfrac{1}{\pi}\int_{0}^{\pi}{x^2dx}=\dfrac{\pi^2}{3}\\
\shoveleft c_n=-c_n \implies \text{for all }x\in [-\pi, \pi], x^2=c_0+\sum_{n=1}^{\infty}{c_n(e^{inx}+e^{-inx})}=\dfrac{\pi^2}{3}+\sum_{n=1}^{\infty}{4\dfrac{(-1)^n}{n^2}cos(nx)}\\
\shoveleft \text{Furthermore, Parseval's identity says that }|c_0|^2+\sum_{n=1}^{\infty}{(|c_n|^2+|-c_n|^2)}=\dfrac{1}{2\pi}\int_{-\pi}^{\pi}{|x^2|^2dx}\\
\shoveleft \implies \dfrac{\pi^4}{9}+2\sum_{n=1}^{\infty}{\frac{4}{n^4}}=\dfrac{1}{\pi}\int_{0}^{\pi}{x^4dx}=\dfrac{1}{\pi}\dfrac{\pi^5}{5}=\dfrac{\pi^4}{5}\implies \zeta(4)=\sum_{n=1}^{\infty}{\dfrac{1}{n^4}}=\dfrac{\pi^4}{8}(\dfrac{1}{5}-\dfrac{1}{9})=\bbox[5px, border: 1px solid black]{\dfrac{\pi^4}{90}}
\end{multline}
$$
**Solve 2:**
$$
\begin{multline}\nonumber
\shoveleft \text{Without using } Parseval's identity \text{, starting from Euler's approach:}\\
\shoveleft \text{Euler devides the infinite power series } sin\theta=\frac{\theta}{1!}-\frac{\theta^3}{3!}+\frac{\theta^5}{5!}-\frac{\theta^7}{7!}+... \text{ by }y=sin\theta:\\
\shoveleft 0=1-\dfrac{\theta}{1!y}+\dfrac{\theta^3}{3!y}-\dfrac{\theta^5}{5!y}+\dfrac{\theta^7}{7!y}-...=(1-\dfrac{\theta}{\theta_0})(1-\dfrac{\theta}{\theta_1})(1-\dfrac{\theta}{\theta_2})(1-\dfrac{\theta}{\theta_3})(1-\dfrac{\theta}{\theta_4})...\\
\shoveleft \text{where the infinitely many roots }\theta_0, \theta_1, \theta_2,...\text{ are the angles for which }sin\theta_n=y=sin\theta.\\
\shoveleft \text{Coefficients on each power of }\theta \text{ on both sides gives the respective powers of }\theta, \theta^2, \theta^3, \theta^4:\\
\shoveleft \text{Then check the values for }y=sin\theta=1, \theta_0=\frac{\pi}{2}:\\
\shoveleft \dfrac{1}{1!y}=\dfrac{1}{\theta_0}+\dfrac{1}{\theta_1}+\dfrac{1}{\theta_2}+\dfrac{1}{\theta_3}+...=\dfrac{1}{\theta_0}+\dfrac{1}{\pi-\theta_0}+\dfrac{1}{-\pi-\theta_0}+\dfrac{1}{-2\pi+\theta_0}+\dfrac{1}{2\pi+\theta_0}+...\implies \\
\shoveleft 1=\dfrac{1}{\tfrac{\pi}{2}}+\dfrac{1}{\pi-\tfrac{\pi}{2}}+\dfrac{1}{-\pi-\tfrac{\pi}{2}}+\dfrac{1}{-2\pi+\tfrac{\pi}{2}}+\dfrac{1}{2\pi+\tfrac{\pi}{2}}+...=\dfrac{2}{\pi}\Big(\dfrac{1}{1}+\dfrac{1}{1}-\dfrac{1}{3}-\dfrac{1}{3}+\dfrac{1}{5}+\dfrac{1}{5}-...\Big)\\
\shoveleft 0=\dfrac{1}{\theta_0\theta_1}+\dfrac{1}{\theta_0\theta_2}+\dfrac{1}{\theta_0\theta_3}+\dfrac{1}{\theta_0\theta_4}+\dfrac{1}{\theta_1\theta_2}+\dfrac{1}{\theta_1\theta_3}+\dfrac{1}{\theta_1\theta_4}+\dfrac{1}{\theta_2\theta_3}+\dfrac{1}{\theta_2\theta_4}+\dfrac{1}{\theta_3\theta_4}...\\
\shoveleft -\dfrac{1}{3!y}=\dfrac{1}{6}=\dfrac{1}{\theta_0\theta_1\theta_2}+\dfrac{1}{\theta_0\theta_1\theta_3}+\dfrac{1}{\theta_0\theta_1\theta_4}+\dfrac{1}{\theta_0\theta_2\theta_3}+\dfrac{1}{\theta_0\theta_2\theta_4}+\dfrac{1}{\theta_0\theta_3\theta_4}+\dfrac{1}{\theta_1\theta_2\theta_3}+\dfrac{1}{\theta_1\theta_2\theta_4}+...\\
\shoveleft 0=\dfrac{1}{\theta_0\theta_1\theta_2\theta_3}+\dfrac{1}{\theta_0\theta_1\theta_2\theta_4}+\dfrac{1}{\theta_0\theta_1\theta_3\theta_4}+\dfrac{1}{\theta_0\theta_2\theta_3\theta_4}+\dfrac{1}{\theta_1\theta_2\theta_3\theta_4}+...\\
\shoveleft \text{Euler expresses the sum of fourth powers of terms in an arbitrary series }a,b,c,d,e,... \text{ as}\\
\shoveleft a^4+b^4+c^4+d^4+e^4+... = \alpha^4 -4\alpha^2 \beta +4\alpha\gamma + 2\beta^2-4\delta \text{, where} \\
\shoveleft \alpha=a+b+c+d+e+...=\dfrac{2}{\pi}\Big(1+1-\dfrac{1}{3}-\dfrac{1}{3}+\dfrac{1}{5}+\dfrac{1}{5}-...\Big) \implies\\
\shoveleft a=\dfrac{1}{\theta_0}=\dfrac{2}{\pi}=b=\dfrac{1}{\theta_1}, c=\dfrac{1}{\theta_2}=-\dfrac{2}{\pi}\dfrac{1}{3}=-\dfrac{2}{3\pi}=d=\dfrac{1}{\theta_4}, e=\dfrac{1}{\theta_5}=\dfrac{2}{\pi}\dfrac{1}{5}=\dfrac{2}{5\pi},...\\
\shoveleft \beta=ab+ac+ad+ae+bc+bd+be+cd+ce+de+... \\
\shoveleft \gamma=abc+abd+abe+acd+ace+ade+bcd+bce+cde+... \\
\shoveleft \delta=abcd+abce+abde+acde+bcde+... \\
\shoveleft \implies a^4+b^4+c^4+d^4+e^4+...=\dfrac{16}{\pi^4}\Big(1+1+\dfrac{1}{3^4}+\dfrac{1}{3^4}+\dfrac{1}{5^4}+\dfrac{1}{5^4}+...\Big)=1^4-\dfrac{4}{6}=\dfrac{1}{3}\\
\shoveleft \implies \sum_{n=1,3,5,...}^{\infty}{\dfrac{1}{n^4}}=\dfrac{1}{1^4}+\dfrac{1}{3^4}+\dfrac{1}{5^4}+\dfrac{1}{7^4}+...=\dfrac{\pi^4}{96}\\
\shoveleft \implies \sum_{n=1,2,3...}^{\infty}{\Big(\dfrac{1}{1^4}+\dfrac{1}{2^4}+\dfrac{1}{3^4}+\dfrac{1}{4^4}+...\Big)}=\dfrac{16}{15}\dfrac{15}{16}\Big(\dfrac{1}{1^4}+\dfrac{1}{2^4}+\dfrac{1}{3^4}+\dfrac{1}{4^4}+...\Big)\\
\shoveleft =\dfrac{16}{15}\Big(1-\dfrac{1}{2^4}\Big)\Big(\dfrac{1}{1^4}+\dfrac{1}{2^4}+\dfrac{1}{3^4}+\dfrac{1}{4^4}+...\Big)\\
\shoveleft =\dfrac{16}{15}\Big(\dfrac{1}{1^4}+\dfrac{1}{2^4}+\dfrac{1}{3^4}+\dfrac{1}{4^4}+...-\dfrac{1}{2^4}-\dfrac{1}{4^4}-\dfrac{1}{6^4}-\dfrac{1}{8^4}-...\Big)\\
\shoveleft =\dfrac{16}{15}\Big(\dfrac{1}{1^4}+\dfrac{1}{3^4}+\dfrac{1}{5^4}+\dfrac{1}{7^4}+...\Big)=\dfrac{16}{15}\dfrac{\pi^4}{96}=\bbox[5px, border: 1px solid black]{\dfrac{\pi^4}{90}}
\end{multline}
$$
**Note:**

- [Parseval's identity Approach](/assets/files/parseval_identity/fourier_example.pdf)

- [Euler's approach explanation](/assets/files/parseval_identity/sum_of_fourth_powers_of_reciprocal_natural_numbers.pdf)

- [Euler's paper: On the sums of series of reciprocals](/assets/files/parseval_identity/on_the_sums_of_series_of_reciprocals.pdf)

- [Calculating Infinite Series Using Parseval's Identity](/assets/files/parseval_identity/calculating_infinite_series_using_parsevals_identity.pdf)

- In Chapter 5-6 of [INSTITUTIONUM CALCULI DIFFERENTIALIS](https://www.17centurymaths.com/contents/differentialcalculus.htm), Euler proved that $\zeta(2n)=\displaystyle\sum_{k=1}^{+\infty}{\dfrac{1}{k^{2n}}}=(-1)^{n-1}\dfrac{(2\pi)^{2n}\cdot B_{2n}}{2(2n)!}$, for $n\in \mathbb{N}$, where $B_{2n}$ denotes the Bernoulli numbers, defined by $B_0=1, B_n=\displaystyle\sum_{s=0}^{n}{ {n \choose s} B_s}$, for $n \le 2$.

  ---

### 11/20/2023

#### $AB=AC, \angle{CAB}=90^{\circ}$ for $\triangle{ABC}$. $D$ is inside $\triangle{ABC}$ such that $\angle{ADB}=90^{\circ}$, $[ADC]=25$, $[BCD]=84$, find $[ADB]$.

![image-20231120134852451](/assets/images/2023/image-20231120134814414.png)

**Solve:**

![image-20231120140142842](/assets/images/2023/image-20231120140142842.png)
$$
\begin{multline}\nonumber
\shoveleft \text{Make } DE\perp AB \text{ at }E, DF\perp AC \text{ at }F, \text{ let }AB=AC=a, DF=m, DE=n\\
\shoveleft \implies AE=m, BE=a-m, n^2=m(a-m), \dfrac{am}{2}=25, \dfrac{a^2}{2}-\dfrac{am}{2}-\dfrac{an}{2}=84\\
\shoveleft \implies am=50, an=a^2-218, 2500+(a^2-218)^2=50a^2 \implies a^4-486a^2+50024=0\\
\shoveleft \implies a^2=338 \text{ or } 148 \implies a=\sqrt{338} \text{ (}a=\sqrt{148} \text{ is abandoned}) \implies [ABD]=\dfrac{an}{2}=\bbox[5px, border: 1px solid black]{60}
\end{multline}
$$
**Solve 2:**

![image-20231120125805676](/assets/images/2023/image-20231120125805676.png)
$$
\begin{multline}\nonumber
\shoveleft \text{Make } CE\perp DB \text{ at }E, CF\perp AD \text{ at }F, \text{ let }AB=AC=a, DE=m, DF=n\\
\shoveleft \implies \angle{ABD}=\angle{CAD}=\angle{ACE}\implies ABCE\text{ is cyclic}\implies \angle{AEB}=45^{\circ}\\
\shoveleft \implies AD=m=CF \implies \triangle{ACF}\cong\triangle{BAD}\implies BD=m+n\\
\shoveleft \implies \dfrac{m^2}{2}=25 \implies m=5\sqrt{2} \implies \dfrac{(m+n)n}{2}=84 \implies n=7\sqrt{2}\\
\shoveleft \implies [ABD]=\dfrac{m(m+n)}{2}=\bbox[5px, border: 1px solid black]{60}
\end{multline}
$$

---

### 11/21/2023

#### $\odot{O_1}, \odot{O_2}$ are two circles tangent to each other at $E$ and are inscribed in segment of $\odot{O}$ and its secant $AB$. $P,Q$ are the tangent points of $\odot{O_1}, \odot{O_2}$ on $AB$, show that $\angle{AEP}=\angle{BEQ}$.

![image-20231123031957455](/assets/images/2023/image-20231123031957455.png)

**Prove:**

![image-20231123033957290](/assets/images/2023/image-20231123033744100.png)
$$
\begin{multline}\nonumber
\shoveleft \text{Let } M,N \text{ be the tangent points of }\odot{O_1},\odot{O_2} \text{ with }\odot{O}\\
\shoveleft CED \text{ be the tangent line of }\odot{O_!}, \odot{O_2} \text{ and intersect with } \odot{O}\text{ at } C, D\\
\shoveleft \text{The structure of inscribed circles in circular segments has some properties:}\\
\shoveleft AC=BC, E \text{ is the incenter of }\triangle{ABD}:  \text{details can be checked at the notes below.}\\
\shoveleft \implies \angle{CAP}=\angle{AMC}=\angle{ADC}=\angle{CDB}=\angle{CNB}=\angle{ABC}=\angle{2}\\
\shoveleft \angle{QPE}=\angle{PEC}=\angle{PME}=\angle{1}, \angle{PQE}=\angle{CEQ}=\angle{ENQ}=\angle{3}\\
\shoveleft \angle{DAE}=\angle{EAP}=\angle{5}, \angle{DBE}=\angle{EBQ}=\angle{6}\\
\shoveleft \angle{1}=\angle{5}+\angle{AEP}, \angle{2}+\angle{5}=\angle{1}+\angle{AEP}\implies \angle{2}=2\angle{AEP}\\
\shoveleft \angle{3}=\angle{6}+\angle{BEQ}, \angle{2}+\angle{6}=\angle{3}+\angle{BEQ}\implies \angle{2}=2
\angle{BEQ}\\
\shoveleft \implies \angle{AEP}=\angle{BEQ}\blacksquare
\end{multline}
$$

**Notes:**

- There are some other properties easy to be proved: $MPQN$ is cyclic, $PE\perp EQ$.
- [Cut-the-knot](https://www.cut-the-knot.org/Curriculum/Geometry/IncircleInSegment.shtml) has some explanations on the topic of circles inscribed in circular segments.
- [Here](https://publications.azimpremjiuniversity.edu.in/2022/1/Circles%20Inscribed%20in%20Segments_At%20Right%20Angle%20July%2019.pdf) is the online copy of the best resource on this topic, and [here](/assets/files/inscribed-circle/circles_inscribed_in_segments_at_right_angle.pdf) is the local copy of this PDF.

---

### 11/30/2023

#### $\odot{O_1}$ is inside $\odot{O}$ and they are tangent at $P$. $AB$ is a secant of $\odot{O}$ and is tangent to $\odot{O_1}$ at $Q$. Prove that the circumcircle of $\triangle{AO_1B}$ bisects $PQ$.

![image-20231130193053857](/assets/images/2023/image-20231130193053857.png)

**Prove:**

![image-20231204070321867](/assets/images/2023/image-20231204070321867.png)
$$
\begin{multline}\nonumber
\shoveleft \text{Let }O_2 \text{ be the center of the circumcircle of }\triangle{AO_1B}\\
\shoveleft \text{Extend }BA \text{ to }T \text{ such that }TP \text{ is tangent to }\odot{O_1} \implies TP\perp PO_1\\
\shoveleft \text{Suppose }R \text{ is the mid point of }PQ \implies TRO_1 \text{ are collinear}, TR \perp PQ\\
\shoveleft \implies TP^2=TR\cdot TO_1\\
\shoveleft \text{For }\odot{O}, TP^2=TA \cdot TB \implies TR \cdot TO_1=TA\cdot TB \implies RABO_1 \text{ are cyclic}\\
\shoveleft \implies R \text{ is on }\odot{O_2} \implies R \text{ is the intersect of }\odot{O_2} \text{ and } PQ \implies PR=QR\blacksquare
\end{multline}
$$
**Note: some conclusions can be got from here:**

* The extended $PQ$ and $O_1O_2$ will intersect on $\odot{O_2}$, let it be $C$
* From previous problem we know that extended $PQ$ and $OO_2$ will intersect on $\odot{O}$, let it be $E$
* $E$ is the midpoint of $\overset{\huge\frown}{AB}$, and is also the midpoint of $QC$

---

