---
title: September 2023
date: 2023-09-01 13:02
tags: []
---

#### 09/01/2023

##### $D, E$ is on side $BC, AC$ of equilateral $\triangle{ABC}$ such that $\angle{ADB}=2\angle{EDC}$. Prove that $AD=BD+CE$.

![image-20230901130602876](/assets/images/2023/image-20230901130602876.png)

**Prove 1:**

![image-20230901130700387](/assets/images/2023/image-20230901130700387.png)
$$
\begin{multline}\nonumber
\shoveleft \text{Let } F \text{ on side } AB \text{ such that } DF \text{ bisects } \angle{ADB}.\\
\shoveleft \text{Let }AB=BC=CA=d, AD=a, BD=b, CD=d-b, CE=c\\
\shoveleft DF \text{ bisects }\angle{ADB} \implies  \dfrac{a}{AF}=\dfrac{b}{BF}\\
\shoveleft \angle{CDE}=\angle{BDF}, \angle{DBF}=\angle{DCE}\implies \triangle{DBF} \sim \triangle{CDE}\\
\shoveleft \implies \dfrac{c}{BF}=\dfrac{d-b}{b} \implies BF=\dfrac{bc}{d-b}, AF=\dfrac{ac}{d-b}\\
\shoveleft \implies AB=d=\dfrac{(a+b)c}{d-b} \implies d(d-b)=(a+b)c\\
\shoveleft cos(\angle{ABD})=\dfrac{d^2+b^2-a^2}{2bd}=cos(60^{\circ})=\dfrac{1}{2} \implies d^2 + b^2 - a^2 = bd\\
\shoveleft \implies (a+b)(a-b)=d(d-b) = (a+b)c \implies a=b+c \implies AD=BD+CE \blacksquare
\end{multline}
$$
**Prove 2:**

![image-20230902113649928](/assets/images/2023/image-20230902113649928.png)
$$
\begin{multline}\nonumber
\shoveleft \text{Rotate } \triangle{ABD} \text{ 60 degrees clockwise around } B \text{ to get } \triangle{CBF}\\
\shoveleft \text{Let } G \text{ on } CF \text{ such that }\angle{CDG}=\alpha, \text{connect } DG, EG\\
\shoveleft \implies \angle{BFC=2\alpha}, CF=AD, \triangle{BDF} \text{ is equilateral} \implies BD=BF=DF\\
\shoveleft \implies \angle{DFG}=2\alpha-60^{\circ}, \angle{FDG}=120^{\circ}-\alpha \\
\shoveleft \implies \angle{FGD}=\angle{FDG}=180^{\circ}-(60^{\circ}+\alpha)=\angle{DEC}\\
\shoveleft \implies BD=DF=FG, CEDG \text{ is cyclic}\\
\shoveleft \implies \angle{CGE}=\angle{CDE}=\alpha, \angle{CEG}=\angle{CDG}=\alpha\\
\shoveleft \implies CE=CG \implies CF=GF+CG=BD+CE=AD\blacksquare\\
\end{multline}
$$
**Prove 3:**

![image-20230902120848800](/assets/images/2023/image-20230902120848800.png)
$$
\begin{multline}\nonumber
\shoveleft \text{Rotate } \triangle{ABD} \text{ 60 degrees counter-clockwise around } A \text{ to get } \triangle{ACF}\\
\shoveleft \text{Extend } FC \text{ to } G \text{ such that } \angle{CDG}=\alpha \implies \triangle{ADF} \text{ is equilateral}\\
\shoveleft BD=CF, \angle{FDC}=120^{\circ}-2\alpha,\angle{DCG}=60^{\circ} \implies CG=CE,\angle{FGD}=120^{\circ}-\alpha\\
\shoveleft \implies \angle{FGD}=\angle{FDG} \implies AD=FD=FG \implies FG=AD=BD+CE\blacksquare
\end{multline}
$$

#### 09/10/2023

##### In trapezoid $ABCD$,$BC \parallel AD$, $M, N$ are two points inside it such that $AM \parallel CN, BN \parallel DM$. Prove that $[ABN]=[CDM]$.

![image-20230910171142140](/assets/images/2023/image-20230910171142140.png)

**Prove:**

![image-20230910173458519](/assets/images/2023/image-20230910173458519.png)
$$
\begin{multline}\nonumber
\shoveleft [ABN]=[ABC]-[ACN]-[BCN], [ABC]=[DBC], [ACN]=[MCN]\\
\shoveleft \implies [ABN]=[DBC]-[MCN]-[BCN]=[BDN]+[DCN]-[MCN]\\
\shoveleft [BDN]=[MDN] \implies [ABN]=[MDN]+[DCN]-[MCN]\\
\shoveleft =[CDMN]-[MCN]=[MCN]+[CDM]-[MCN]=[CDM]\blacksquare
\end{multline}
$$

---

#### 09/11/2023

#### $D, E$ are points on side $AC, BC$ in right-angle $\triangle{ABC}$ such that $\angle{BDE}=90^{\circ}, \angle{DBE}=\angle{CDE}, [ABD]=[CDE]=1$, find $[BDE]$.

![image-20230911045009257](/assets/images/2023/image-20230911045009257.png)

**Solve:**

![image-20230911050905435](/assets/images/2023/image-20230911050046200.png)
$$
\begin{multline}\nonumber
\shoveleft \text{Let } G \text{ on } BC \text{ such that } DG\perp BC, F \text{ on extended } DE \text{ such that } DF \perp CF\\
\shoveleft \implies \angle{GDE}=\angle{DBE}=\angle{ABD}=\angle{CDE}=\angle{ECF}=\angle{\alpha}\\
\shoveleft \text{Let } GE=a, DG=b, [ABD]=[CDE]=1\implies\\
\shoveleft  b^3=2a,AD=GD=b, AB=GB=\dfrac{b^2}{a}, DE=\sqrt{a^2+b^2}, CF=\dfrac{2}{\sqrt{a^2+b^2}}\\
\shoveleft \implies \dfrac{DG}{GE}=\dfrac{DE+EF}{CF}\implies \dfrac{b}{a}=\dfrac{\sqrt{a^2+b^2}+\dfrac{2a}{b\sqrt{a^2+b^2}}}{\dfrac{2}{\sqrt{a^2+b^2}}} \implies\\
\shoveleft a^3+ab^2+\dfrac{2a^2}{b}=2b \implies a^3b^3+ab^5+2a^2b^2=2b^4\implies (ab)^3+2a^2b^2+2a^2b^2=4ab\\
\shoveleft \implies (ab)^2+4ab=4 \implies ab=\sqrt{2}-1\implies [BDE]=1+ab=\bbox[5px, border: 1px solid black]{\sqrt{2}}
\end{multline}
$$
**Solve 2:**
$$
\begin{multline}\nonumber
\shoveleft \text{Let } G \text{ on } BC \text{ such that } DG\perp BC, [DGE]=x \implies\\
\shoveleft \angle{GDE}=\angle{DBE}=\angle{ABD}=\angle{CDE}=\angle{ECF}=\angle{\alpha}\implies\\
\shoveleft AD=DG,\dfrac{[BCD]}{[ABD]}=\dfrac{2+x}{1}=\dfrac{CD}{AD}=\dfrac{CD}{DG}=\dfrac{CE}{GE}=\dfrac{[CDE]}{[GDE]}=\dfrac{1}{x}\\
\shoveleft \implies x^2+2x-1=0\implies x=\sqrt{2}-1\implies [BDE]=\bbox[5px, border: 1px solid black]{\sqrt{2}}
\end{multline}
$$

---

