---
title: July 2023
date: 2023-07-26 05:16
tags: []

---

### 07/26/2023

#### There are $a_1, a_2, \dots, a_m \in \{ 1, 2, \dots, m \}$, $b_1, b_2, \dots, b_m \in \{ 1, 2, \dots, m \}$. Prove that there exists $1 \le p \le q \le m$ and $1 \le s \le t \le m$ such that $a_p + \dots + a_q = b_s + \dots + b_t$ (from 2023 Beijing NCEE)

**Prove:**
$$
\begin{multline}\nonumber
\shoveleft \text{Let } A_i = a_1 + a_2 + \dots + a_i, B_i = b_1 + b_2 + \dots + b_m, (1 \le i \le m), A_0=B_0=0.\\
\shoveleft \text{And Let } r_k=max\{ i | B_i \le A_k, k \in \{0, 1, \dots, m\}\}\\
\shoveleft \text{Without Loss of Generality, we assume } A_m \ge B_m. \text{ Let } S_k = A_k - B_{r_k} \text{ for }1 \le k \le m \implies S_k \ge 0.\\
\shoveleft \text{From the definition of } r_k \implies A_k-B_{r_k+1} < 0 \implies b_{r_k+1}=B_{r_k+1}-B_{r_k}= S_k - (A_k-B_{r_k+1})\\
\shoveleft b_{r_k+1} \in \{1,2, \dots, m\} \implies b_{r_k+1} \le m \implies S_k \le m + (A_k - B_{r_k+1}) \lt m \implies S_k \le m-1\\
\shoveleft \text{If } \exists k \text{ such that } S_k=0 \implies r=p=1, q=k,s=r_k, a_1+\dots+a_q=A_k=B_{r_k}=b_1+\cdots+b_{r_k}\blacksquare\\
\shoveleft \text{If } \nexists k \text{ such that }S_k=0 \implies S_k \in \{ 1,2,\dots, m-1 \} \text{ for } k \in \{ 1,2, \dots, m\} \\
\shoveleft \implies \exists 1 \le u \lt v \le m \text{ such that } S_u=S_v \implies A_u-B_{r_u}=A_v-B_{r_v} \implies A_v-A_u=B_{r_v}-B_{r_u}\\
\shoveleft \implies p=v-u+1, q=v, s=r_v-r_u+1, t=r_v, a_{v-u+1}+\dots+a_v=b_{r_v-r_u+1}+\dots+b_{r_v}\blacksquare\\
\shoveleft \text{Similarly the conclusion holds when } B_m \ge A_m. \text{ Done. }\blacksquare  \\
\end{multline}\\
$$
