---
title: February 2024
date: 2024-02-12 20:44
tags: []
---

### 02/12/2024

#### Points $$D,E,F$$ are on side $$BC, CA, AB$$ of acute triangle $$\triangle{ABC}$$ respectively such that $$DE \perp AC, EF \perp AB, FD \perp BC$$. Prove that $$\tfrac{AF}{AB}+\tfrac{BD}{BC}+\tfrac{CE}{CA}=1$$

![image-20240212115039732](/assets/images/2024/image-20240212115039732.png)

**Prove 1:**

![image-20240212160636085](/assets/images/2024/image-20240212155937058.png)
$$
\begin{multline}\nonumber
\shoveleft \text{Make }AP \perp BC \text{ at }P, BQ \perp CA \text{ at }Q, CR \perp AB \text{ at }R\\
\shoveleft AP, BQ, CR \text{ intersect at }H, \text{ connect }DH, EH, \text{ and } FH\\
\shoveleft [AFC]=[AEF]+[CEF],[CEF]=[HEF]\\
\shoveleft [ABD]=[BDF]+[ADF],[ADF]=[HDF]\\
\shoveleft [BCE]=[CDE]+[BDE],[BDE]=[HDE]\\
\shoveleft [HEF]+[HDF]+[HDE]=[DEF]\implies\\
\shoveleft [AFC]+[ABD]+[BCE]=[AEF]+[BDF]+[CDE]+[DEF]\\
\shoveleft =[ABC] \implies \dfrac{AF}{AB}+\dfrac{BD}{BC}+\dfrac{CE}{CA}\\
\shoveleft =\dfrac{AF\cdot CR}{AB \cdot CR}+\dfrac{BD \cdot AP}{BC \cdot AP}+\dfrac{CE \cdot BQ}{CA \cdot BQ}\\
\shoveleft =\dfrac{[AFC]+[ABD]+[BCE]}{[ABC]}=\dfrac{[ABC]}{[ABC]}=1\blacksquare\\
\end{multline}
$$
**Prove 2:**

![image-20240212162625073](/assets/images/2024/image-20240212162625073.png)
$$
\begin{multline}
\shoveleft \text{Let }M, N \text{ on }CA \text{ such that }FM \parallel BC, DN \parallel AB\\
\shoveleft \angle{ABC}=90^{\circ}-\angle{BFD}=\angle{DFE}, \angle{BCA}=90^{\circ}-\angle{CDE}=\angle{EDF}\\
\shoveleft \implies \triangle{DEF}\sim\triangle{ABC}\implies \dfrac{DE}{EF}=\dfrac{CA}{AB}=\dfrac{AM}{AF}\\
\shoveleft DN \parallel AB, EF \perp AB \implies DN \perp EF \implies\\
\shoveleft \angle{EDN}=90^{\circ}-\angle{DEF}=\angle{AEF}\implies \triangle{AEF}\sim\triangle{NDE}\\
\shoveleft \implies \dfrac{DE}{EF}=\dfrac{NE}{AF}\implies \dfrac{NE}{AF}=\dfrac{AM}{AF}\\
\shoveleft \implies NE=AM \implies AN=ME\\
\shoveleft \implies \dfrac{AF}{AB}+\dfrac{BD}{BC}+\dfrac{CE}{CA}=\dfrac{AM}{CA}+\dfrac{AN}{CA}+\dfrac{CE}{CA}\\
\shoveleft =\dfrac{AM+ME+CE}{CA}=1\blacksquare
\end{multline}
$$

---

### 02/14/2024

#### $$a+\dfrac{1}{b}=x, b+\dfrac{1}{c}=y, c+\dfrac{1}{a}=z, $$ find $$abc$$.

**Solve:**
$$
\begin{multline}
\shoveleft \text{Sum up three equations }\implies a+b+c+\dfrac{1}{a}+\dfrac{1}{b}+\dfrac{1}{c}=x+y+z\\
\shoveleft \text{Multiple three equations }\implies abc+a+b+c+\dfrac{1}{a}+\dfrac{1}{b}+\dfrac{1}{c}+\dfrac{1}{abc}=xyz\\
\shoveleft \implies abc+x+y+z+\dfrac{1}{abc}=xyz\implies (abc)^2+(x+y+z-xyz){abc}+1=0\\
\shoveleft \implies abc=\bbox[5px, border: 1px solid black]{\dfrac{xyz-x-y-z\pm\sqrt{(xyz-x-y-z)^2-4}}{2}}
\end{multline}
$$

---

### 02/15/2024

#### $$x+\dfrac{1}{x}=3$$, find $$\dfrac{x^6+1}{x^5+x}$$

**Solve:**
$$
\begin{multline}
\shoveleft x+\dfrac{1}{x}=3 \implies x^2+\dfrac{1}{x^2}=(x+\dfrac{1}{x})^2-2=7\\
\shoveleft \implies x^3+\dfrac{1}{x^3}=(x+\dfrac{1}{x})(x^2-1+\dfrac{1}{x^2})=3*6=18\\
\shoveleft \implies \dfrac{x^6+1}{x^5+x}=\dfrac{x^3+\dfrac{1}{x^3}}{x^2+\dfrac{1}{x^2}}=\bbox[5px, border: 1px solid black]{\dfrac{18}{7}}
\end{multline}
$$

---

### 02/18/2024

#### $$\dfrac{x}{y+z}+\dfrac{y}{z+x}+\dfrac{z}{x+y}=1$$, find $$\dfrac{x^2}{y+z}+\dfrac{y^2}{z+x}+\dfrac{z^2}{x+y}$$

**Solve:**
$$
\begin{multline}
\shoveleft (\dfrac{x}{y+z}+\dfrac{y}{z+x}+\dfrac{z}{x+y})(x+y+z)\\
\shoveleft =\dfrac{x^2}{y+z}+\dfrac{y^2}{z+x}+\dfrac{z^2}{x+y}+x+y+z\\
\shoveleft \implies \dfrac{x^2}{y+z}+\dfrac{y^2}{z+x}+\dfrac{z^2}{x+y}=\bbox[5px, border: 1px solid black]{0}
\end{multline}
$$

---

### 02/20/2024

#### $$a+b+c=0, \dfrac{1}{a+1}+\dfrac{1}{b+2}+\dfrac{1}{c+3}=0$$, find $$(a+1)^2+(b+2)^2+(c+3)^2$$

**Solve:**
$$
\begin{multline}
\shoveleft \text{Let }x=a+1, y=b+2, z=c+3 \implies x+y+z=6\\
\shoveleft \dfrac{1}{a+1}+\dfrac{1}{b+2}+\dfrac{1}{c+3}=0 \implies \dfrac{1}{x}+\dfrac{1}{y}+\dfrac{1}{z}=0\\
\shoveleft \implies xy+yz+zx=0 \implies x^2+y^2+z^2=(x+y+z)^2\\
\shoveleft \implies x^2+y^2+z^2=(a+1)^2+(b+2)^2+(c+3)^2=\bbox[5px, border: 1px solid black]{36}
\end{multline}
$$

---

### 02/21/2024

#### $$abc \neq 0, a+b+c=0$$, find $$\dfrac{a^2}{bc}+\dfrac{b^2}{ca}+\dfrac{c^2}{ab}$$

**Solve:**
$$
\begin{multline}
\shoveleft (a+b+c)^3=a^3+b^3+c^3+6abc+3[ab(a+b)+bc(b+c)+ca(c+a)]\\
\shoveleft  a+b+c=0\implies (a+b+c)^3=a^3+b^3+c^3-3abc=0, abc \neq 0\\
\shoveleft \implies \dfrac{a^3+b^3+c^3}{abc}=3\implies \dfrac{a^2}{bc}+\dfrac{b^2}{ca}+\dfrac{c^2}{ab}=\bbox[5px, border: 1px solid black]{3}
\end{multline}
$$

---

