---
title: October 2024
date: 2024-10-04 05:03
tags: []
---

### 10/04/2024

#### $D$ is a point inside $\triangle{ABC}$ such that $\angle{ABD}=6^{\circ}$, $\angle{BAD}=30^{\circ}$, $\angle{CAD}=54^{\circ}$, $\angle{ACD}=24^{\circ}$, find $\angle{CBD}$.

![image-20241004050430794](/assets/images/2024/image-20241004050430794.png)

**Solve:**

![image-20241005044451477](/assets/images/2024/image-20241004050848572.png)
$$
\begin{multline}
\shoveleft \text{Extend }CD \text{ to }E \text{ such that }AC=AE \implies \angle{AEC}=\angle{ACE}=24^{\circ}, \angle{EAB}=48^{\circ}\\
\shoveleft \implies \angle{EDA}=78^{\circ}=\angle{EAD}\implies EA=ED=AC, \angle{EDB}=66^{\circ}\\
\shoveleft \text{Let }F \text{ on }AB \text{ such that }\angle{DEF}=60^{\circ}\implies \angle{AEF}=84^{\circ}\implies \angle{AFE}=48^{\circ}=\angle{EAB}\\
\shoveleft \implies EF=EA=ED\implies \triangle{DEF}\text{ is equilateral}\implies \angle{EFD}=\angle{EDF}=60^{\circ}\\
\shoveleft DF=EF=DE=EA=AC\implies \angle{AFD}=12^{\circ}\implies \angle{BDF}=6^{\circ}=\angle{ABD}\\
\shoveleft \implies BF=DF=EF\implies \angle{EBF}=\angle{BEF}=24^{\circ}=\angle{ACD}\implies ACBE\text{ is cyclic}\\
\shoveleft \implies \angle{ABC}=\angle{AEC}=24^{\circ}\implies \angle{CBD}=24^{\circ}-6^{\circ}=\bbox[5px, border: 1px solid black]{18^{\circ}}
\end{multline}
$$

---

### 10/06/2024

#### $D$ is a point inside $\triangle{ABC}$ such that $\angle{BAD}=20^{\circ}$, $\angle{CAD}=30^{\circ}$, $\angle{ACD}=40^{\circ}$, $\angle{BCD}=10^{\circ}$, find $\angle{CBD}$.

![image-20241006213056781](/assets/images/2024/image-20241006213056781.png)

**Solve:**

![image-20241006212924216](/assets/images/2024/image-20241006212924216.png)
$$
\begin{multline}
\shoveleft \angle{BAC}=50^{\circ}=\angle{BCA}\implies AB=BC, \angle{ABC}=80^{\circ}\\
\shoveleft \text{Extend }AD \text{ to }E \text{ such that }AB=BE\implies \angle{BEA}=\angle{BAE}=20^{\circ}\\
\shoveleft \implies \angle{ABE}=140^{\circ}\implies \angle{EBC}=60^{\circ}\\
\shoveleft AB=BE=BC\implies \triangle{BCE} \text{ is equilateral} \implies BE=EC=BC=AE\\
\shoveleft \angle{BEC}=60^{\circ}=\angle{BCE}\implies \angle{DEC}=40^{\circ},\angle{DCE}=70^{\circ}\\
\shoveleft \implies \angle{CDE}=70^{\circ}=\angle{DCE}\implies CE=DE=BE\implies \angle{DBE}=80^{\circ}\\
\shoveleft \implies \angle{CBD}=\angle{DBE}-\angle{EBC}=\bbox[5px, border: 1px solid black]{20^{\circ}}
\end{multline}
$$

---

### 10/07/2024

#### $\triangle{ABC}$ is an isosceles triangle with $AB=AC$, $\angle{ABC}=\angle{ACB}=80^{\circ}$, $D$ is inside $\triangle{ABC}$ such that $\angle{ABD}=50^{\circ}$, $\angle{ACD}=25^{\circ}$ , find $\angle{CAD}$.

![image-20241011010646279](/assets/images/2024/image-20241011010646279.png)

**Solve:**

![image-20241011005649038](/assets/images/2024/image-20241011005649038.png)

$$
\begin{multline}
\shoveleft AB=AC\implies \angle{ABC}=\angle{ABC}=80^{\circ}\implies  \angle{BAC}=20^{\circ}\\
\shoveleft \text{Extend } BD \text{ to }E \text{ such that }AB=AE \implies\\
\shoveleft \angle{ABE}=\angle{AEB}=50^{\circ}, \angle{BAE}=80^{\circ} \implies \\
\shoveleft \angle{CAE}=60^{\circ}\implies \triangle{CAE} \text{ is equilateral} \implies\\
\shoveleft \angle{ACE}=\angle{AEC}=60^{\circ}\implies \angle{BEC}=10^{\circ}, \angle{ECD}=85^{\circ}=\angle{EDC}\\
\shoveleft \implies EC=ED=AE, \angle{AED}=50^{\circ}\implies \angle{ADE}=\angle{DAE}=65^{\circ}\\
\shoveleft \implies \angle{CAD}=\angle{DAE}-60^{\circ}=\bbox[5px, border: 1px solid black]{5^{\circ}}
\end{multline}
$$

---

### asdas

#### asdsa

![image-20241010054600395](/assets/images/2024/image-20241010054600395.png)
$$
\begin{multline}
\shoveleft [BHF]=\dfrac{AH}{AD}[BDF], [CDH]=\dfrac{BH}{BE}[CDE], [AEH]=\dfrac{CH}{CF}[AEF]\\
\shoveleft [AHF]=\dfrac{BH}{BE}[AEF], [BDH]=\dfrac{CH}{CF}[BDF], [CHE]=\dfrac{AH}{AD}[CDE]\\
\shoveleft \implies (\dfrac{AH}{AD}+\dfrac{CH}{CF})[BDF]+(\dfrac{BH}{BE}+\dfrac{AH}{AD})[CDE]+(\dfrac{CH}{CF}+\dfrac{BH}{BE})[AEF]\\
\shoveleft =[ABC]=[BDF]+[CDE]+[AEF]+[DEF] \implies [DEF]=\\
\shoveleft (\dfrac{AH}{AD}+\dfrac{CH}{CF}-1)[BDF]+(\dfrac{BH}{BE}+\dfrac{AH}{AD}-1)[CDE]+(\dfrac{CH}{CF}+\dfrac{BH}{BE}-1)[AEF]\\
\shoveleft \dfrac{AH}{AD}+\dfrac{CH}{CF}-1=\dfrac{AH}{AD}-\dfrac{FH}{CF}=\dfrac{\dfrac{AH \cdot CF}{AD}-FH}{CF}=\dfrac{\dfrac{AH \cdot BC}{BD}-FH}{CF}=\dfrac{\dfrac{FH \cdot CD}{BD}}{CF}=\dfrac{CF \cdot DH}{CF \cdot BD}=\dfrac{DH}{BD}\\
\shoveleft \dfrac{BH}{BE}+\dfrac{AH}{AD}-1=\dfrac{BH}{BE}-\dfrac{DH}{AD}=\dfrac{\dfrac{BH \cdot AC}{BC}-DH}{AD}=\dfrac{\dfrac{DH \cdot AC}{CE}-DH}{AD}=\dfrac{\dfrac{AE\cdot DH}{CE}}{AD}=\dfrac{}{CE}
\end{multline}
$$
