---
title: May 2024
date: 2024-05-01 17:45
tags: []
---

### 05/01/2024

#### $\angle{BAC}=16^{\circ}, \angle{CAD}=22^{\circ}, \angle{ABD}=38^{\circ}, \angle{CBD}=44^{\circ}$ in quadrilateral $ABCD$, find $\angle{ACD}$.

![image-20240501174742108](/assets/images/2024/image-20240501174742108.png)

**Solve:**

![image-20240501174659614](/assets/images/2024/image-20240501174659614.png)
$$
\begin{multline}
\shoveleft \text{Easy to see that }\angle{DAB}=\angle{DBA}=38^{\circ}\implies AD=BD, \angle{ADB}=104^{\circ}, \angle{ACB}=82^{\circ}\\
\shoveleft \text{Extend }BC \text{ to }E \text{ such that } \angle{DAE}=8^{\circ} \implies \angle{CAE}=30^{\circ}\implies \angle{AEC}=52^{\circ}=\dfrac{\angle{ADB}}{2}\\
\shoveleft \implies D\text{ is the circumcenter of }\triangle{ABE} \implies AD=DE=DB, \angle{AED}=\angle{DAE}=8^{\circ}\\
\shoveleft \text{Let }F \text{ be the reflection of }E \text{ along line }AC \implies \angle{CAF}=\angle{CAE}=30^{\circ},AE=AF, CE=CF\\
\shoveleft \text{Connect }AF, CF\implies \triangle{AEF} \text{ is equilateral triangle} \implies \angle{CEF}=\angle{CFE}=8^{\circ}=\angle{DAE}\\
\shoveleft \implies \triangle{DAE}\cong\triangle{CEF}\implies DE=CE\implies \angle{ECD}=\angle{EDC}=\dfrac{180^{\circ}-44^{\circ}}{2}=68^{\circ}\\
\shoveleft \implies \angle{ACD}=180^{\circ}-82^{\circ}-68^{\circ}=\bbox[5px, border: 1px solid black]{30^{\circ}}
\end{multline}
$$

---

### 05/02/2024

#### Factorize $x^6-4x^3-1$

**Solve:**
$$
\begin{multline}
\shoveleft \text{Suppose there is }a \text{ such that } x^6-4x^3-1=x^6-ax^3+(a-4)x^3-1\\
\shoveleft =x^3(x^3-a)+(a-4)x^3-1 \text{ and we hope }\dfrac{1}{a}=\dfrac{a-4}{1}=k\\
\shoveleft  \implies a^2-4a-1=0\implies a=2\pm \sqrt{5} \implies a-4=-2\pm\sqrt{5}\\
\shoveleft \implies k=\dfrac{1}{2\pm\sqrt{5}}=\dfrac{2\mp\sqrt{5}}{-1}=-2\pm\sqrt{5}\\
\shoveleft \implies x^6-4x^3-1=x^6-ax^3+kx^3-ak=(x^3+k)(x^3-a)\\
\shoveleft =\bbox[5px, border: 1px solid black]{(x^3-2+\sqrt{5})(x^3-2-\sqrt{5})}\\
\end{multline}
$$

---

### 05/08/2024

#### Solve cubic equation: $x^3=3ax^2+6bx+2c$

**Solve:**
$$
\begin{multline}
\shoveleft x^3=3ax^2+6bx+2c\\
\shoveleft \text{Let }x=y+a \implies (y+a)^3=3a(y+a)^2+6b(y+a)+2c\\
\shoveleft \implies y^3+3ay^2+3a^2y+a^3=3ay^2+6a^2y+3a^3+6by+6ab+2c\\
\shoveleft \implies y^3=3(a^2+2b)y+2(a^3+3ab+c)\\
\shoveleft \text{Let }p=a^2+2b, q=a^3+3ab+c \implies y^3=3py+2q\\
\shoveleft u_1=q+\sqrt[3]{q^2-p^3}, u_2=q-\sqrt[3]{q^2-p^3}\\
\shoveleft \omega_1=\dfrac{-1+\sqrt{3}i}{2}, \omega_2=\omega_1^2=\dfrac{-1-\sqrt{3}i}{2}\\
\shoveleft \begin{bmatrix}
y_1 \\ y_2 \\ y_3
\end{bmatrix}=
\begin{bmatrix}
1 & 1\\
\omega & \omega^2\\
\omega^2 & \omega
\end{bmatrix}
\cdot
\begin{bmatrix}
u_1 \\ u_2
\end{bmatrix}
\implies
\begin{bmatrix}
x_1 \\ x_2 \\ x_3
\end{bmatrix}=
\begin{bmatrix}
1 & 1 & 1\\
\omega & \omega^2 & 1\\
\omega^2 & \omega & 1
\end{bmatrix} \cdot
\begin{bmatrix}
u_1 \\ u_2 \\ a
\end{bmatrix}
=
\begin{bmatrix}
u_1+u_2+a\\
\omega_1\cdot u_1+\omega_2\cdot u_2+a\\
\omega_2 \cdot u_1 + \omega_1 \cdot u_2+a\\
\end{bmatrix}\\
\shoveleft \text{Summary: }\\
\shoveleft x^3=3ax^2+6bx+2c \implies\\
\shoveleft p=a^2+2b, q=a^3+3ab+c\\
\shoveleft u_1=q+\sqrt[3]{q^2-p^3}, u_2=q-\sqrt[3]{q^2-p^3}\\
\shoveleft \implies
\begin{bmatrix}
x_1 \\ x_2 \\ x_3
\end{bmatrix}=
\begin{bmatrix}
1 & 1 & 1\\
\omega & \omega^2 & 1\\
\omega^2 & \omega & 1
\end{bmatrix} \cdot
\begin{bmatrix}
u_1 \\ u_2 \\ a
\end{bmatrix}
\end{multline}
$$

**Note:**
$$
\begin{multline}
\shoveleft \text{Quadratic equation:}\\
\shoveleft x^2=2px+q \implies x=p \pm \sqrt{p^2+q}\\
\end{multline}
$$




---

### 05/10/2024

#### $D$ is a point inside $\triangle{ABC}$ such that $\angle{BAD}=72^{\circ}$, $\angle{CAD}=24^{\circ}$, $\angle{CBD}=6^{\circ}$, find $\angle{BCD}$.

![image-20240510001103151](/assets/images/2024/image-20240510001103151.png)

**Solve:**

![image-20240510002531941](/assets/images/2024/image-20240510001016944.png)
$$
\begin{multline}
\shoveleft \text{Easy to see that }\\
\shoveleft \angle{ACB}=42^{\circ}=\angle{ABC}\implies AB=AC\\
\shoveleft \angle{ADB}=72^{\circ}=\angle{BAD}\implies AB=BD\\
\shoveleft \text{Make }E\text{ on bisector of }\angle{BAD} \text{ such that }AB=AE\\
\shoveleft \implies \triangle{ABE}\cong\triangle{ABD}, \angle{AEB}=\angle{ABE}=72^{\circ}\\
\shoveleft \implies ABED \text{ are cyclic} \implies \angle{AED}=\angle{ABD}=36^{\circ}\\
\shoveleft \angle{EAC}=60^{\circ}, AE=AB=AC\implies \triangle{ACE}\text{ is equilateral}\\
\shoveleft \implies AC=CE, \angle{AEC}=60^{\circ}\implies \angle{CED}=24^{\circ}=\angle{CAD}\\
\shoveleft \implies \triangle{CAD}\cong\triangle{CED} \implies \angle{ACD}=\angle{ECD}=30^{\circ}\\
\shoveleft \implies \angle{BCD}=42^{\circ}-30^{\circ}=\bbox[5px, border: 1px solid black]{12^{\circ}}\\
\end{multline}
$$


